Cleanup and documentation

execution/theories/ContractMorphisms.v
@@ -23,19 +23,16 @@ Definition curry_fun3 {A B C D : Type} (f : A * B * C -> D) : A -> B -> C -> D :
     fun (a : A) => fun (b : B) => fun (c : C) => f (a,b,c).
 Definition uncurry_fun3 {A B C D : Type} (f : A -> B -> C -> D) : A * B * C -> D :=
     fun (x : A * B * C) => 
-        let (x', c) := x in 
-        let (a, b) := x' in f a b c.
+        let '(a, b, c) := x in f a b c.
 Definition curry_fun4 {A B C D E : Type} (f : A * B * C * D -> E) : A -> B -> C -> D -> E :=
     fun (a : A) => fun (b : B) => fun (c : C) => fun (d : D) => f (a,b,c,d).
 Definition uncurry_fun4 {A B C D E : Type} (f : A -> B -> C -> D -> E) : A * B * C * D -> E :=
     fun (x : A * B * C * D) => 
-        let (x' , d) := x in 
-        let (x'', c) := x' in 
-        let (a, b) := x'' in f a b c d.
+        let '(a, b, c, d) := x in f a b c d.
 Definition serialize_function {A B} `{Serializable A} `{Serializable B} 
     (f : A -> B) (sv : SerializedValue) : SerializedValue := 
     match deserialize sv with 
-    | None => sv (* should not be deserializable *)
+    | None => sv (* ideally would not be deserializable *)
     | Some a => serialize (f a)
     end.
 Definition option_fun {A B} (f : A -> B) (op_a : option A) : option B := 
@@ -44,15 +41,84 @@ Definition option_fun {A B} (f : A -> B) (op_a : option A) : option B :=
     | None => None 
     end.
 
+
 Section ContractMorphisms.
 Context { Base : ChainBase }.
 
-
+(** First, a definition of a Contract Morphism, which is a function between contracts *)
 Section MorphismDefinition.
-(* TODO amounts do not change with morphisms *)
-(* TODO the actionbody outputs do not change with morphisms. JUST THE STATE. *)
 
-(* init component *)
+(** The init component *)
+Record InitCM
+    { Setup Setup' Msg Msg' State State' Error Error' : Type }
+    `{Serializable Msg}  `{Serializable Setup}  `{Serializable State}  `{Serializable Error}
+    `{Serializable Msg'} `{Serializable Setup'} `{Serializable State'} `{Serializable Error'}
+    (C : Contract Setup Msg State Error) (C' : Contract Setup' Msg' State' Error') 
+    := build_init_cm {
+        (* transform inputs/outputs of the init function *)
+        init_inputs : Chain * ContractCallContext * Setup -> 
+            Chain * ContractCallContext * Setup' ;
+        init_outputs : result State Error -> result State' Error' ;
+        (* proof of commutativity *)
+        init_commutes : 
+            forall x : Chain * ContractCallContext * Setup,
+                uncurry_fun3 C'.(init) (init_inputs x) = 
+                init_outputs (uncurry_fun3 C.(init) x) ;
+    }.
+
+(** The receive component *)
+Record RecvCM
+    { Setup Setup' Msg Msg' State State' Error Error' : Type }
+    `{Serializable Msg}  `{Serializable Setup}  `{Serializable State}  `{Serializable Error}
+    `{Serializable Msg'} `{Serializable Setup'} `{Serializable State'} `{Serializable Error'}
+    (C : Contract Setup Msg State Error) (C' : Contract Setup' Msg' State' Error') := 
+    build_recv_cm {
+        (* transform inputs/outputs of the receive function *)
+        recv_inputs : Chain * ContractCallContext * State * option Msg -> 
+            Chain * ContractCallContext * State' * option Msg' ;
+        recv_outputs : result (State * list ActionBody) Error -> 
+            result (State' * list ActionBody) Error' ;
+        (* proof of commutativity *)
+        recv_commutes : 
+            forall (x : Chain * ContractCallContext * State * option Msg), 
+                uncurry_fun4 C'.(receive) (recv_inputs x) = 
+                recv_outputs (uncurry_fun4 C.(receive) x) ;
+    }.
+
+(** The definition *)
+Record ContractMorphism 
+    { Setup Setup' Msg Msg' State State' Error Error' : Type }
+    `{Serializable Msg}  `{Serializable Setup}  `{Serializable State}  `{Serializable Error}
+    `{Serializable Msg'} `{Serializable Setup'} `{Serializable State'} `{Serializable Error'}
+    (C  : Contract Setup  Msg  State  Error) 
+    (C' : Contract Setup' Msg' State' Error') := 
+    build_cm {
+        cm_init : InitCM C C' ;
+        cm_recv : RecvCM C C' ;
+    }.
+
+End MorphismDefinition.
+
+
+Section MorphismUtilities.
+
+Definition init_cm 
+    { Setup Setup' Msg Msg' State State' Error Error' : Type }
+    `{Serializable Msg}  `{Serializable Setup}  `{Serializable State}  `{Serializable Error}
+    `{Serializable Msg'} `{Serializable Setup'} `{Serializable State'} `{Serializable Error'}
+    {C : Contract Setup Msg State Error} {C' : Contract Setup' Msg' State' Error'} 
+    (f : ContractMorphism C C') : InitCM C C' := 
+    cm_init C C' f.
+Definition recv_cm 
+        { Setup Setup' Msg Msg' State State' Error Error' : Type }
+        `{Serializable Msg}  `{Serializable Setup}  `{Serializable State}  `{Serializable Error}
+        `{Serializable Msg'} `{Serializable Setup'} `{Serializable State'} `{Serializable Error'}
+        {C : Contract Setup Msg State Error} {C' : Contract Setup' Msg' State' Error'} 
+    (f : ContractMorphism C C') : RecvCM C C' := 
+    cm_recv C C' f.
+Definition id_fun (A : Type) : A -> A := @id A.
+
+(* the coherence conditions for constructing non-opaque morphisms *)
 Definition init_morphs_commute  
     { Setup Setup' State State' Error Error' : Type}
     (init  : Chain -> ContractCallContext -> Setup  -> result State  Error)
@@ -64,22 +130,6 @@ Definition init_morphs_commute
         uncurry_fun3 init' (init_inputs x) = 
         init_outputs (uncurry_fun3 init x).
 
-Record InitCM
-    { Setup Setup' Msg Msg' State State' Error Error' : Type }
-    `{Serializable Msg}  `{Serializable Setup}  `{Serializable State}  `{Serializable Error}
-    `{Serializable Msg'} `{Serializable Setup'} `{Serializable State'} `{Serializable Error'}
-    (C : Contract Setup Msg State Error) (C' : Contract Setup' Msg' State' Error') 
-    (* takes input a state morphism *)
-    := build_initcm {
-        init_inputs : Chain * ContractCallContext * Setup -> 
-            Chain * ContractCallContext * Setup' ;
-        init_outputs : result State Error -> result State' Error' ;
-        (* proof of diagram commutativity *)
-        init_commutes : 
-            init_morphs_commute C.(init) C'.(init) init_inputs init_outputs ;
-    }.
-
-(* recv component *)
 Definition recv_morphs_commute 
     { Msg Msg' State State' Error Error' : Type }
     (recv  : Chain -> ContractCallContext -> State  -> option Msg  -> 
@@ -94,68 +144,46 @@ Definition recv_morphs_commute
             uncurry_fun4 recv' (recv_inputs x) = 
             recv_outputs (uncurry_fun4 recv x).
 
-Record RecvCM
-    { Setup Setup' Msg Msg' State State' Error Error' : Type }
-    `{Serializable Msg}  `{Serializable Setup}  `{Serializable State}  `{Serializable Error}
-    `{Serializable Msg'} `{Serializable Setup'} `{Serializable State'} `{Serializable Error'}
-    (* takes input a state morphism and an actionbody morphism *)
-    (C : Contract Setup Msg State Error) (C' : Contract Setup' Msg' State' Error') := {
-        recv_inputs : Chain * ContractCallContext * State * option Msg -> 
-            Chain * ContractCallContext * State' * option Msg' ;
-        recv_outputs : result (State * list ActionBody) Error -> 
-            result (State' * list ActionBody) Error' ;
-        (* proof of diagram commutativity *)
-        recv_commutes : 
-            recv_morphs_commute C.(receive) C'.(receive) recv_inputs recv_outputs ;
-    }.
-
-(* definition *)
-Record ContractMorphism 
-        { Setup Setup' Msg Msg' State State' Error Error' : Type }
-        `{Serializable Msg}  `{Serializable Setup}  `{Serializable State}  `{Serializable Error}
-        `{Serializable Msg'} `{Serializable Setup'} `{Serializable State'} `{Serializable Error'}
-    (* uses the same state morphism (and same actionbody morphism) *)
-    (C  : Contract Setup  Msg  State  Error) 
-    (C' : Contract Setup' Msg' State' Error') := {
-        cm_init : InitCM C C' ;
-        cm_recv : RecvCM C C' ;
-    }.
-
-End MorphismDefinition.
-
-
-Section MorphismUtilities.
-
-Definition init_cm 
-        { Setup Setup' Msg Msg' State State' Error Error' : Type }
-        `{Serializable Msg}  `{Serializable Setup}  `{Serializable State}  `{Serializable Error}
-        `{Serializable Msg'} `{Serializable Setup'} `{Serializable State'} `{Serializable Error'}
-        {C : Contract Setup Msg State Error} {C' : Contract Setup' Msg' State' Error'} 
-    (f : ContractMorphism C C') : InitCM C C' := 
-    cm_init C C' f.
-Definition recv_cm 
-        { Setup Setup' Msg Msg' State State' Error Error' : Type }
-        `{Serializable Msg}  `{Serializable Setup}  `{Serializable State}  `{Serializable Error}
-        `{Serializable Msg'} `{Serializable Setup'} `{Serializable State'} `{Serializable Error'}
-        {C : Contract Setup Msg State Error} {C' : Contract Setup' Msg' State' Error'} 
-    (f : ContractMorphism C C') : RecvCM C C' := 
-    cm_recv C C' f.
-Definition id_morph (A : Type) : A -> A := @id A.
-
 End MorphismUtilities.
 
 
-(* The Identity Contract Morphism *)
+(** The Identity Contract Morphism *)
 Section IdentityMorphism.
 
+(* an opaque construction *)
+Definition id_cm_opaque 
+    { Setup Msg State Error : Type }
+    `{Serializable Msg}  `{Serializable Setup}  `{Serializable State} `{Serializable Error}
+    (C : Contract Setup Msg State Error) : ContractMorphism C C.
+Proof.
+    constructor.
+    -   set (init_inputs  := id_fun (Chain * ContractCallContext * Setup)).
+        set (init_outputs := id_fun (result State Error)).
+        apply (build_init_cm Setup Setup Msg Msg State State Error Error H H0 H1 H2 H H0 H1 H2 C C init_inputs init_outputs).
+        intro. destruct x. destruct p.
+        unfold uncurry_fun3. 
+        unfold init_inputs. unfold init_outputs. 
+        unfold id_fun. simpl.
+        reflexivity.
+    -   set (recv_inputs  := id_fun (Chain * ContractCallContext * State * option Msg)).
+        set (recv_outputs := id_fun (result (State * list ActionBody) Error)).
+        apply (build_recv_cm Setup Setup Msg Msg State State Error Error H H0 H1 H2 H H0 H1 H2 C C recv_inputs recv_outputs).
+        intro. destruct x. repeat destruct p.
+        unfold uncurry_fun4. 
+        unfold recv_inputs. unfold recv_outputs. 
+        unfold id_fun. simpl.
+        reflexivity.
+Qed.
+
+(* an explicity construction *)
 Lemma init_commutes_id 
     { Setup Msg State Error : Type }
     `{Serializable Msg}  `{Serializable Setup}  `{Serializable State} `{Serializable Error}
     (C : Contract Setup Msg State Error) :
     init_morphs_commute 
         C.(init) C.(init) 
-        (id_morph (Chain * ContractCallContext * Setup)) 
-        (id_morph (result State Error)).
+        (id_fun (Chain * ContractCallContext * Setup)) 
+        (id_fun (result State Error)).
 Proof. intro. auto. Qed.
 
 Definition id_cm_init 
@@ -163,30 +191,30 @@ Definition id_cm_init
     `{Serializable Msg}  `{Serializable Setup}  `{Serializable State} `{Serializable Error}
     (C : Contract Setup Msg State Error) :
     InitCM C C := {|
-        init_inputs  := id_morph (Chain * ContractCallContext * Setup) ;
-        init_outputs := id_morph (result State Error) ;
+        init_inputs  := id_fun (Chain * ContractCallContext * Setup) ;
+        init_outputs := id_fun (result State Error) ;
         (* proof of commutativity *)
         init_commutes := init_commutes_id C ;
     |}.
 
-Lemma r_commutes_id 
+Lemma recv_commutes_id 
     { Setup Msg State Error : Type }
     `{Serializable Msg}  `{Serializable Setup}  `{Serializable State} `{Serializable Error}
     (C : Contract Setup Msg State Error) :
     recv_morphs_commute 
         C.(receive) C.(receive) 
-        (id_morph (Chain * ContractCallContext * State * option Msg)) 
-        (id_morph (result (State * list ActionBody) Error)).
+        (id_fun (Chain * ContractCallContext * State * option Msg)) 
+        (id_fun (result (State * list ActionBody) Error)).
 Proof. intro. auto. Qed.
 
 Definition id_cm_recv 
-        { Setup Msg State Error : Type }
-        `{Serializable Msg}  `{Serializable Setup}  `{Serializable State} `{Serializable Error}
+    { Setup Msg State Error : Type }
+    `{Serializable Msg}  `{Serializable Setup}  `{Serializable State} `{Serializable Error}
     (C : Contract Setup Msg State Error) : RecvCM C C := {|
-        recv_inputs := id_morph (Chain * ContractCallContext * State * option Msg) ;
-        recv_outputs := id_morph (result (State * list ActionBody) Error) ;
+        recv_inputs := id_fun (Chain * ContractCallContext * State * option Msg) ;
+        recv_outputs := id_fun (result (State * list ActionBody) Error) ;
         (* proof of commutativity *)
-        recv_commutes := r_commutes_id C ;
+        recv_commutes := recv_commutes_id C ;
     |}.
 
 (* * the identity morphism *)
@@ -200,14 +228,14 @@ Definition id_cm
 
 End IdentityMorphism.
 
-(* Deriving Equality of Contract Morphisms *)
+(** Deriving equality of Contract Morphisms *)
 Section EqualityOfMorphisms.
 
 Lemma is_eq_cm 
-        { Setup Setup' Msg Msg' State State' Error Error' : Type }
-        `{Serializable Msg}  `{Serializable Setup}  `{Serializable State}  `{Serializable Error}
-        `{Serializable Msg'} `{Serializable Setup'} `{Serializable State'} `{Serializable Error'}
-        {C : Contract Setup Msg State Error} {C' : Contract Setup' Msg' State' Error'} :
+    { Setup Setup' Msg Msg' State State' Error Error' : Type }
+    `{Serializable Msg}  `{Serializable Setup}  `{Serializable State}  `{Serializable Error}
+    `{Serializable Msg'} `{Serializable Setup'} `{Serializable State'} `{Serializable Error'}
+    {C : Contract Setup Msg State Error} {C' : Contract Setup' Msg' State' Error'} :
     forall (f g : ContractMorphism C C'), 
     init_cm f = init_cm g -> 
     recv_cm f = recv_cm g -> 
@@ -221,11 +249,11 @@ Proof.
       exact recv_eq.
 Qed.
 
-Lemma is_eq_cm_init  
-        { Setup Setup' Msg Msg' State State' Error Error' : Type }
-        `{Serializable Msg}  `{Serializable Setup}  `{Serializable State}  `{Serializable Error}
-        `{Serializable Msg'} `{Serializable Setup'} `{Serializable State'} `{Serializable Error'}
-        {C : Contract Setup Msg State Error} {C' : Contract Setup' Msg' State' Error'} :
+Lemma is_eq_cm_init
+    { Setup Setup' Msg Msg' State State' Error Error' : Type }
+    `{Serializable Msg}  `{Serializable Setup}  `{Serializable State}  `{Serializable Error}
+    `{Serializable Msg'} `{Serializable Setup'} `{Serializable State'} `{Serializable Error'}
+    {C : Contract Setup Msg State Error} {C' : Contract Setup' Msg' State' Error'} :
     forall (f g : ContractMorphism C C'),
     (init_inputs C C' (init_cm f)) = (init_inputs C C' (init_cm g)) -> 
     (init_outputs C C' (init_cm f)) = (init_outputs C C' (init_cm g)) -> 
@@ -238,10 +266,10 @@ Proof.
 Qed.
 
 Lemma is_eq_cm_recv 
-        { Setup Setup' Msg Msg' State State' Error Error' : Type }
-        `{Serializable Msg}  `{Serializable Setup}  `{Serializable State}  `{Serializable Error}
-        `{Serializable Msg'} `{Serializable Setup'} `{Serializable State'} `{Serializable Error'}
-        {C : Contract Setup Msg State Error} {C' : Contract Setup' Msg' State' Error'} :
+    { Setup Setup' Msg Msg' State State' Error Error' : Type }
+    `{Serializable Msg}  `{Serializable Setup}  `{Serializable State}  `{Serializable Error}
+    `{Serializable Msg'} `{Serializable Setup'} `{Serializable State'} `{Serializable Error'}
+    {C : Contract Setup Msg State Error} {C' : Contract Setup' Msg' State' Error'} :
     forall (f g : ContractMorphism C C'),
     (recv_inputs C C' (recv_cm f)) = (recv_inputs C C' (recv_cm g)) -> 
     (recv_outputs C C' (recv_cm f)) = (recv_outputs C C' (recv_cm g)) -> 
@@ -256,16 +284,18 @@ Qed.
 End EqualityOfMorphisms.
 
 
+(** An explicit construction of the composition of two morphisms *)
 Section MorphismComposition.
 
+(** The Init component *)
 Lemma compose_commutes_init 
-        { Setup Setup' Setup'' Msg Msg' Msg'' State State' State'' Error Error' Error'' : Type }
-        `{Serializable Msg}    `{Serializable Setup}    `{Serializable State}    `{Serializable Error}
-        `{Serializable Msg'}   `{Serializable Setup'}   `{Serializable State'}   `{Serializable Error'}
-        `{Serializable Msg''}  `{Serializable Setup''}  `{Serializable State''}  `{Serializable Error''}
-        { C : Contract Setup Msg State Error } 
-        { C' : Contract Setup' Msg' State' Error' }
-        { C'' : Contract Setup'' Msg'' State'' Error'' } 
+    { Setup Setup' Setup'' Msg Msg' Msg'' State State' State'' Error Error' Error'' : Type }
+    `{Serializable Msg}    `{Serializable Setup}    `{Serializable State}    `{Serializable Error}
+    `{Serializable Msg'}   `{Serializable Setup'}   `{Serializable State'}   `{Serializable Error'}
+    `{Serializable Msg''}  `{Serializable Setup''}  `{Serializable State''}  `{Serializable Error''}
+    { C : Contract Setup Msg State Error } 
+    { C' : Contract Setup' Msg' State' Error' }
+    { C'' : Contract Setup'' Msg'' State'' Error'' } 
     (g : ContractMorphism C' C'')
     (f : ContractMorphism C  C') :
     init_morphs_commute 
@@ -280,14 +310,15 @@ Proof.
     reflexivity.
 Qed.
 
+(** The Recv component *)
 Lemma compose_commutes_recv
-        { Setup Setup' Setup'' Msg Msg' Msg'' State State' State'' Error Error' Error'' : Type }
-        `{Serializable Msg}    `{Serializable Setup}    `{Serializable State}    `{Serializable Error}
-        `{Serializable Msg'}   `{Serializable Setup'}   `{Serializable State'}   `{Serializable Error'}
-        `{Serializable Msg''}  `{Serializable Setup''}  `{Serializable State''}  `{Serializable Error''}
-        { C : Contract Setup Msg State Error } 
-        { C' : Contract Setup' Msg' State' Error' }
-        { C'' : Contract Setup'' Msg'' State'' Error'' } 
+    { Setup Setup' Setup'' Msg Msg' Msg'' State State' State'' Error Error' Error'' : Type }
+    `{Serializable Msg}    `{Serializable Setup}    `{Serializable State}    `{Serializable Error}
+    `{Serializable Msg'}   `{Serializable Setup'}   `{Serializable State'}   `{Serializable Error'}
+    `{Serializable Msg''}  `{Serializable Setup''}  `{Serializable State''}  `{Serializable Error''}
+    { C : Contract Setup Msg State Error } 
+    { C' : Contract Setup' Msg' State' Error' }
+    { C'' : Contract Setup'' Msg'' State'' Error'' } 
     (g : ContractMorphism C' C'')
     (f : ContractMorphism C  C') :
     recv_morphs_commute 
@@ -302,14 +333,15 @@ Proof.
     reflexivity.
 Qed.
 
+(** Composition *)
 Definition composition_cm 
-        { Setup Setup' Setup'' Msg Msg' Msg'' State State' State'' Error Error' Error'' : Type }
-        `{Serializable Msg}    `{Serializable Setup}    `{Serializable State}    `{Serializable Error}
-        `{Serializable Msg'}   `{Serializable Setup'}   `{Serializable State'}   `{Serializable Error'}
-        `{Serializable Msg''}  `{Serializable Setup''}  `{Serializable State''}  `{Serializable Error''}
-        { C : Contract Setup Msg State Error } 
-        { C' : Contract Setup' Msg' State' Error' }
-        { C'' : Contract Setup'' Msg'' State'' Error'' } 
+    { Setup Setup' Setup'' Msg Msg' Msg'' State State' State'' Error Error' Error'' : Type }
+    `{Serializable Msg}    `{Serializable Setup}    `{Serializable State}    `{Serializable Error}
+    `{Serializable Msg'}   `{Serializable Setup'}   `{Serializable State'}   `{Serializable Error'}
+    `{Serializable Msg''}  `{Serializable Setup''}  `{Serializable State''}  `{Serializable Error''}
+    { C : Contract Setup Msg State Error } 
+    { C' : Contract Setup' Msg' State' Error' }
+    { C'' : Contract Setup'' Msg'' State'' Error'' } 
     (g : ContractMorphism C' C'')
     (f : ContractMorphism C  C') : ContractMorphism C C'' := 
     let compose_init := {|
@@ -329,13 +361,12 @@ Definition composition_cm
         cm_recv := compose_recv ;
     |}.
 
-
-(* Composition with the Identity morphism is trivial *)
+(** Composition with the Identity morphism is trivial *)
 Proposition composition_id_cm_left 
-        { Setup Setup' Msg Msg' State State' Error Error' : Type }
-        `{Serializable Msg}  `{Serializable Setup}  `{Serializable State}  `{Serializable Error}
-        `{Serializable Msg'} `{Serializable Setup'} `{Serializable State'} `{Serializable Error'}
-        {C : Contract Setup Msg State Error} {C' : Contract Setup' Msg' State' Error'} :
+    { Setup Setup' Msg Msg' State State' Error Error' : Type }
+    `{Serializable Msg}  `{Serializable Setup}  `{Serializable State}  `{Serializable Error}
+    `{Serializable Msg'} `{Serializable Setup'} `{Serializable State'} `{Serializable Error'}
+    {C : Contract Setup Msg State Error} {C' : Contract Setup' Msg' State' Error'} :
     forall (f : ContractMorphism C C'), 
     (composition_cm (id_cm C') f) = f.
 Proof.
@@ -346,10 +377,10 @@ Proof.
 Qed.
 
 Proposition composition_id_cm_right 
-        { Setup Setup' Msg Msg' State State' Error Error' : Type }
-        `{Serializable Msg}  `{Serializable Setup}  `{Serializable State}  `{Serializable Error}
-        `{Serializable Msg'} `{Serializable Setup'} `{Serializable State'} `{Serializable Error'}
-        {C : Contract Setup Msg State Error} {C' : Contract Setup' Msg' State' Error'} :
+    { Setup Setup' Msg Msg' State State' Error Error' : Type }
+    `{Serializable Msg}  `{Serializable Setup}  `{Serializable State}  `{Serializable Error}
+    `{Serializable Msg'} `{Serializable Setup'} `{Serializable State'} `{Serializable Error'}
+    {C : Contract Setup Msg State Error} {C' : Contract Setup' Msg' State' Error'} :
     forall (f : ContractMorphism C C'), 
     (composition_cm f (id_cm C)) = f.
 Proof.
@@ -359,24 +390,24 @@ Proof.
     + apply (is_eq_cm_recv (composition_cm f (id_cm C)) f); auto.
 Qed.
 
-(* Composition is Associative *)
+(** Composition is associative *)
 Proposition composition_assoc_cm 
-        { Setup Setup' Setup'' Setup''' 
-        Msg   Msg'   Msg''   Msg''' 
-        State State' State'' State''' 
-        Error Error' Error'' Error''' : Type }
-        `{Serializable Msg} `{Serializable Setup} `{Serializable State} `{Serializable Error}
-        `{Serializable Msg'} `{Serializable Setup'} `{Serializable State'} `{Serializable Error'}
-        `{Serializable Msg''} `{Serializable Setup''} `{Serializable State''} `{Serializable Error''}
-        `{Serializable Msg'''} `{Serializable Setup'''} `{Serializable State'''} `{Serializable Error'''}
-        { C : Contract Setup Msg State Error } 
-        { C' : Contract Setup' Msg' State' Error' }
-        { C'' : Contract Setup'' Msg'' State'' Error'' }
-        { C''' : Contract Setup''' Msg''' State''' Error''' } :
+    { Setup Setup' Setup'' Setup''' 
+    Msg   Msg'   Msg''   Msg''' 
+    State State' State'' State''' 
+    Error Error' Error'' Error''' : Type }
+    `{Serializable Msg} `{Serializable Setup} `{Serializable State} `{Serializable Error}
+    `{Serializable Msg'} `{Serializable Setup'} `{Serializable State'} `{Serializable Error'}
+    `{Serializable Msg''} `{Serializable Setup''} `{Serializable State''} `{Serializable Error''}
+    `{Serializable Msg'''} `{Serializable Setup'''} `{Serializable State'''} `{Serializable Error'''}
+    { C : Contract Setup Msg State Error } 
+    { C' : Contract Setup' Msg' State' Error' }
+    { C'' : Contract Setup'' Msg'' State'' Error'' }
+    { C''' : Contract Setup''' Msg''' State''' Error''' } :
     forall 
-        (f : ContractMorphism C C') 
-        (g : ContractMorphism C' C'') 
-        (h : ContractMorphism C'' C'''), 
+    (f : ContractMorphism C C') 
+    (g : ContractMorphism C' C'') 
+    (h : ContractMorphism C'' C'''), 
     composition_cm h (composition_cm g f) =
     composition_cm (composition_cm h g) f.
 Proof.
@@ -395,727 +426,7 @@ Qed.
 End MorphismComposition.
 
 
-Section SimpleContractMorphism.
-(* contract morphisms can be constructed by *)
-
-Definition simple_cm_construct 
-        { Setup Setup' Msg Msg' State State' Error Error' : Type }
-        `{Serializable Msg}  `{Serializable Setup}  `{Serializable State}  `{Serializable Error}
-        `{Serializable Msg'} `{Serializable Setup'} `{Serializable State'} `{Serializable Error'}
-        {C1 : Contract Setup Msg State Error} {C2 : Contract Setup' Msg' State' Error'}
-    (msg_morph   : Msg   -> Msg')
-    (setup_morph : Setup -> Setup')
-    (state_morph : State -> State')
-    (* TODO plus some coherence conditions *)
-    : ContractMorphism C1 C2 := todo "".
-
-End SimpleContractMorphism.
-
-Section ContractMorphismLift.
-Context 
-    (* we can lift a morphism of contracts, parameterized by the morphpism f and the address of C1 *)
-    { Setup Setup' Msg Msg' State State' Error Error' : Type }
-    `{Serializable Msg}  `{Serializable Setup}  `{Serializable State}  `{Serializable Error}
-    `{Serializable Msg'} `{Serializable Setup'} `{Serializable State'} `{Serializable Error'}
-    {C1 : Contract Setup Msg State Error} {C2 : Contract Setup' Msg' State' Error'}
-    {f : ContractMorphism C1 C2}
-    (* f must be decomposable as follows *)
-    {msg_morph   : Msg   -> Msg'}
-    {setup_morph : Setup -> Setup'}
-    {state_morph : State -> State'}
-    {f_decomposable : f = simple_cm_construct msg_morph setup_morph state_morph}.
-
-(* TODO *)
-Definition wc_dec_eq : forall w1 w2 : WeakContract, {w1 = w2} + {w1 <> w1} := todo "".
-Declare Scope wc_scope.
-Delimit Scope wc_scope with wc.
-Bind Scope wc_scope with WeakContract.
-Infix "=?" := wc_dec_eq (at level 70) : wc_scope.
-
-(* calls into C1 are transformed into calls into C2
-   deployment of C1 is transformed to deployment of C2 *)
-Definition action_morphism (native_env : Environment) (a : Action) : Action := {| 
-    act_origin := act_origin a ;
-    act_from := act_from a ;
-    act_body := 
-        match act_body a with 
-        (* contract calls into C1 change to calls into C2 *)
-        | act_call to amt msg => 
-            match env_contracts native_env to with 
-            | Some wc => 
-                if (wc =? contract_to_weak_contract C1)%wc
-                then act_call to amt (serialize_function msg_morph msg)
-                else act_body a
-            | None => act_body a
-            end
-        (* we deploy C2 instead of C1 *)
-        | act_deploy amt c setup => 
-            if (c =? contract_to_weak_contract C1)%wc
-            then act_deploy amt (contract_to_weak_contract C2) (serialize_function setup_morph setup)
-            else act_body a
-        (* all amounts stay the same, so we do not change transfers *)
-        | act_transfer _ _ => act_body a 
-        end
-|}.
-
-Record EnvironmentMorphism (e1 e2 : Environment) := 
-    build_env_morphism {
-        chain_eq' : env_chain e1 = env_chain e2 ;
-        account_balances_eq' :
-            forall a, env_account_balances e1 a = env_account_balances e2 a ;
-        contracts_morph :
-            forall a, 
-                env_contracts e2 a = 
-                match env_contracts e1 a with 
-                | Some wc => 
-                    if (wc =? contract_to_weak_contract C1)%wc 
-                    then Some (contract_to_weak_contract C2) 
-                    else Some wc
-                | None => None 
-                end ;
-        contract_states_morph : 
-            forall a, 
-                env_contract_states e2 a = 
-                match env_contracts e1 a with 
-                | Some wc => 
-                    if (wc =? contract_to_weak_contract C1)%wc 
-                    then (option_fun (serialize_function state_morph)) (env_contract_states e1 a)
-                    else env_contract_states e1 a
-                | None => env_contract_states e1 a
-                end ;
-}.
-
-Record ChainStateMorphism (cstate1 cstate2 : ChainState) := 
-    build_chainstate_morphism {
-        env_morph   : EnvironmentMorphism cstate1 cstate2 ;
-        queue_morph : chain_state_queue cstate2 = 
-                      List.map (action_morphism cstate1) (chain_state_queue cstate1) ;
-    }.
-
-(* given a bstate, construct one over f that will (trivially) yield a ChainStateMorphism *)
-Definition bstate_transform_step (bstate : ChainState) : ChainState := 
-        let env := {| 
-            (* the same as bstate *)
-            env_chain := env_chain bstate ; 
-            (* the same as bstate *)
-            env_account_balances := env_account_balances bstate ; 
-            (* the contracts are transformed via the contract morphism *)
-            env_contracts := fun a =>
-                match env_contracts bstate a with 
-                | Some wc => 
-                    if (wc =? contract_to_weak_contract C1)%wc 
-                    then Some (contract_to_weak_contract C2)
-                    else Some wc 
-                | None => None
-                end ;
-            (* the contract states are transformed via the contract morphism *)
-            env_contract_states := fun a => 
-                match env_contracts bstate a with 
-                | Some wc => 
-                    if (wc =? contract_to_weak_contract C1)%wc 
-                    then (option_fun (serialize_function state_morph)) (env_contract_states bstate a)
-                    else env_contract_states bstate a
-                | None => env_contract_states bstate a
-                end ;
-        |} in
-        (* we just use the queue again from bstate1' *)
-        let queue := List.map (action_morphism bstate) (chain_state_queue bstate) in 
-        (* return the new cstate *)
-        {| chain_state_env := env ; chain_state_queue := queue ; |}.
-
-(* the chain_eq' component of an EnvironmentMorphism *)
-Lemma env_morph_step_chain_eq (bstate1 : ChainState) : 
-        let bstate2 := bstate_transform_step bstate1 in
-        env_chain bstate1 = env_chain bstate2.
-Proof. auto. Qed.
-
-(* the account_balances_eq' component of an EnvironmentMorphism *)
-Definition env_morph_step_balances (bstate1 : ChainState) : 
-    let bstate2 := bstate_transform_step bstate1 in
-    forall a, env_account_balances bstate1 a = env_account_balances bstate2 a.
-Proof. auto. Qed.
-
-(* the contract_morphisms component of an EnvironmentMorphism *)
-Definition env_morph_step_contracts (bstate1 : ChainState) :  
-    let bstate2 := bstate_transform_step bstate1 in
-    forall a, 
-        env_contracts bstate2 a = 
-        match env_contracts bstate1 a with 
-        | Some wc => 
-            if (wc =? contract_to_weak_contract C1)%wc 
-            then Some (contract_to_weak_contract C2) 
-            else Some wc
-        | None => None 
-        end.
-Proof. 
-    intros. 
-    unfold bstate2.
-    unfold bstate_transform_step. 
-    simpl. reflexivity.
-Qed.
-
-Definition env_morph_step_states (bstate1 : ChainState) : 
-    let bstate2 := bstate_transform_step bstate1 in
-    forall a,
-        env_contract_states bstate2 a = 
-        match env_contracts bstate1 a with 
-        | Some wc => 
-            if (wc =? contract_to_weak_contract C1)%wc 
-            then (option_fun (serialize_function state_morph)) (env_contract_states bstate1 a)
-            else env_contract_states bstate1 a
-        | None => env_contract_states bstate1 a
-        end.
-Proof.
-    intros.
-    unfold bstate2.
-    unfold bstate_transform_step.
-    simpl. reflexivity.
-Qed.
-
-Definition env_morph_step (bstate1 : ChainState) : 
-    let bstate2 := bstate_transform_step bstate1 in
-    EnvironmentMorphism bstate1 bstate2 := {| 
-        chain_eq' := env_morph_step_chain_eq bstate1 ; 
-        account_balances_eq' := env_morph_step_balances bstate1 ; 
-        contracts_morph := env_morph_step_contracts bstate1 ; 
-        contract_states_morph := env_morph_step_states bstate1 ;
-    |}.    
-
-Lemma queue_morphism_step (bstate1 : ChainState) : 
-    let bstate2 := bstate_transform_step bstate1 in  
-    chain_state_queue bstate2
-    = List.map (action_morphism bstate1) (chain_state_queue bstate1).
-Proof. auto. Qed.
-
-Definition chainstate_morphism_step (bstate1' : ChainState) : 
-    let bstate2' := bstate_transform_step bstate1' in  
-    (ChainStateMorphism bstate1' bstate2') := {|  
-        env_morph   := env_morph_step bstate1' ; 
-        queue_morph := queue_morphism_step bstate1' |}.
-
-
-
-
-
-(* construct the step from bstate2 to bstate2' *)
-Lemma chainstate_morphism_empty_queue 
-    (cstate1 cstate2 : ChainState) 
-    (m : ChainStateMorphism cstate1 cstate2) : 
-    chain_state_queue cstate1 = nil -> chain_state_queue cstate2 = nil.
-Proof. 
-    intro. rewrite (queue_morph cstate1 cstate2 m). rewrite H7. simpl. reflexivity.
-Qed.
-
-Lemma chainstate_morphism_next_block_valid
-    (cstate1 cstate2 : ChainState) 
-    (m : ChainStateMorphism cstate1 cstate2)
-    (header : BlockHeader) : 
-    IsValidNextBlock header cstate1 -> IsValidNextBlock header cstate2.
-Proof.
-    intro. destruct H7.
-    assert (env_chain cstate1 = env_chain cstate2); 
-    try exact (chain_eq' cstate1 cstate2 (env_morph cstate1 cstate2 m)).
-    rewrite H7 in valid_height.
-    rewrite H7 in valid_slot.
-    rewrite H7 in valid_finalized_height. 
-    exact (build_is_valid_next_block header cstate2 valid_height valid_slot valid_finalized_height valid_creator valid_reward).
-Qed.
-
-Lemma chainstate_morphism_no_acts_from_accounts
-    (bstate1' : ChainState) : 
-    let bstate2' := bstate_transform_step bstate1' in  
-    Forall act_is_from_account (chain_state_queue bstate1') -> 
-    Forall act_is_from_account (chain_state_queue bstate2').
-Proof.
-    intros. 
-    unfold bstate2'.
-    simpl.
-    induction (chain_state_queue bstate1').
-    - auto.
-    - simpl. apply Forall_cons_iff in H7. destruct H7. apply IHl in H8.
-        apply Forall_cons.
-        + exact H7.
-        + exact H8.
-Qed.
-
-Lemma chainstate_morphism_origin_eq_from
-    (bstate1' : ChainState) : 
-    let bstate2' := bstate_transform_step bstate1' in  
-    Forall act_origin_is_eq_from (chain_state_queue bstate1') -> 
-    Forall act_origin_is_eq_from (chain_state_queue bstate2').
-Proof.
-    intros. 
-    unfold bstate2'.
-    simpl.
-    induction (chain_state_queue bstate1').
-    - auto.
-    - simpl. apply Forall_cons_iff in H7. destruct H7. apply IHl in H8.
-        apply Forall_cons.
-        + exact H7.
-        + exact H8.
-Qed.
-
-Lemma chainstate_morphism_step_env_chain_eq
-    (bstate1 bstate2 : ChainState)
-    (c_morph : ChainStateMorphism bstate1 bstate2) : 
-    env_chain bstate1 = env_chain bstate2.
-Proof.
-    exact (chain_eq' bstate1 bstate2 (env_morph bstate1 bstate2 c_morph)).
-Qed.
-
-Lemma env_equiv_carries_over_env_morphism 
-    (bstate1 bstate1' bstate2 bstate2' : Environment)
-    (e_morph  : EnvironmentMorphism bstate1  bstate2)
-    (e_morph' : EnvironmentMorphism bstate1' bstate2') :
-    EnvironmentEquiv bstate1 bstate1' -> 
-    EnvironmentEquiv bstate2 bstate2'.
-Proof.
-    intro EE1. destruct EE1. 
-    (* prove chain_eq *)
-    assert (env_chain bstate2 = env_chain bstate2').
-    rewrite (chain_eq' bstate1  bstate2  e_morph)  in chain_eq.
-    rewrite (chain_eq' bstate1' bstate2' e_morph') in chain_eq.
-    exact chain_eq.
-    (* prove account_balances_eq *)
-    assert (forall a, env_account_balances bstate2 a = env_account_balances bstate2' a).
-    intro.
-    rewrite <- (account_balances_eq' bstate1  bstate2  e_morph  a).
-    rewrite <- (account_balances_eq' bstate1' bstate2' e_morph' a).
-    exact (account_balances_eq a).
-    (* prove contracts_eq *)
-    assert (forall a, env_contracts bstate2 a = env_contracts bstate2' a).
-    intro.
-    rewrite (contracts_morph bstate1  bstate2  e_morph  a).
-    rewrite (contracts_morph bstate1' bstate2' e_morph' a).
-    rewrite <- (contracts_eq a). reflexivity.
-    (* prove contract_states_eq *)
-    assert (forall a, env_contract_states bstate2 a = env_contract_states bstate2' a).
-    intro.
-    rewrite (contract_states_morph bstate1  bstate2  e_morph  a).
-    rewrite (contract_states_morph bstate1' bstate2' e_morph' a).
-    rewrite <- (contracts_eq a).
-    rewrite <- (contract_states_eq a). reflexivity.
-    (* construct the result *)
-    exact {| chain_eq := H7 ; 
-             account_balances_eq := H8 ;
-             contracts_eq := H9 ;
-             contract_states_eq := H10 ; |}.
-Qed.
-
-(* then prove that adding a block preserves the cstate morphism *)
-Lemma env_morph_preserved_under_adding_block 
-    (bstate1 bstate2 : ChainState)
-    (e_morph : EnvironmentMorphism bstate1 bstate2)
-    (header : BlockHeader) : 
-    let bstate1' := (add_new_block_to_env header bstate1) in 
-    let bstate2' := (add_new_block_to_env header bstate2) in 
-    EnvironmentMorphism bstate1' bstate2'.
-Proof.
-    intros.
-    (* prove chain_eq' *)
-    assert (env_chain bstate1' = env_chain bstate2'). auto.
-    (* prove account_balances_eq' *)
-    assert (forall a, 
-        env_account_balances bstate1' a = env_account_balances bstate2' a).
-    unfold bstate1'. unfold bstate2'.
-    unfold add_new_block_to_env. 
-    intro. simpl.
-    rewrite <- (account_balances_eq' bstate1 bstate2 e_morph a). reflexivity.
-    (* prove contracts_morph *)
-    assert (forall a, 
-        env_contracts bstate2' a = 
-        match env_contracts bstate1' a with 
-        | Some wc => 
-            if (wc =? contract_to_weak_contract C1)%wc 
-            then Some (contract_to_weak_contract C2) 
-            else Some wc
-        | None => None 
-        end). 
-    unfold bstate1'. unfold bstate2'.
-    unfold add_new_block_to_env. 
-    intro. simpl. 
-    exact (contracts_morph bstate1 bstate2 e_morph a).
-    (* prove contract_states_morph *)
-    assert (forall a, 
-        env_contract_states bstate2' a = 
-        match env_contracts bstate1' a with 
-        | Some wc => 
-            if (wc =? contract_to_weak_contract C1)%wc 
-            then (option_fun (serialize_function state_morph)) (env_contract_states bstate1' a)
-            else env_contract_states bstate1' a
-        | None => env_contract_states bstate1' a
-        end).
-    unfold bstate1'. unfold bstate2'.
-    unfold add_new_block_to_env. 
-    intro. simpl. 
-    exact (contract_states_morph bstate1 bstate2 e_morph a).
-    (* construct the result *)
-    exact {| chain_eq' := H7 ; 
-             account_balances_eq' := H8 ;
-             contracts_morph := H9 ;
-             contract_states_morph := H10 ; |}.
-Qed.
-
-Lemma chainstate_morphism_new_env_equiv_add_block
-    (bstate1 bstate2 bstate1' : ChainState)
-    (e_morph : EnvironmentMorphism bstate1 bstate2) 
-    (header : BlockHeader) : 
-    let bstate2' := bstate_transform_step bstate1' in  
-    EnvironmentEquiv bstate1' (add_new_block_to_env header bstate1) -> 
-    EnvironmentEquiv bstate2' (add_new_block_to_env header bstate2).
-Proof.
-    intros bstate2' EE1.
-    assert (EnvironmentMorphism (add_new_block_to_env header bstate1) (add_new_block_to_env header bstate2)); 
-    try exact (env_morph_preserved_under_adding_block bstate1 bstate2 e_morph header).
-    assert (EnvironmentMorphism bstate1' bstate2');
-    try exact (env_morph_step bstate1').
-    exact (symmetry (env_equiv_carries_over_env_morphism
-        (add_new_block_to_env header bstate1) bstate1'
-        (add_new_block_to_env header bstate2) bstate2'
-        H7 H8  (symmetry EE1))).
-Qed.
-
-Lemma permutation_preserved_over_map {A B : Type} : 
-    forall (g : A -> B) (l1 l2 : list A),
-    Permutation l1 l2 -> 
-    Permutation (List.map g l1) (List.map g l2).
-Proof.
-    intros.
-    induction H7.
-    - auto.
-    - simpl. exact (perm_skip (g x) IHPermutation).
-    - simpl. exact (perm_swap (g x) (g y) (map g l)).
-    - exact (perm_trans IHPermutation1 IHPermutation2).
-Qed.
-
-Lemma chainstate_morphism_new_permuted 
-    (bstate1 bstate2 bstate1' : ChainState)
-    (env_equiv : EnvironmentEquiv bstate1 bstate1') 
-    (c_morph : ChainStateMorphism bstate1 bstate2) : 
-    let bstate2' := bstate_transform_step bstate1' in 
-    Permutation (chain_state_queue bstate1) (chain_state_queue bstate1') -> 
-    Permutation (chain_state_queue bstate2) (chain_state_queue bstate2').
-Proof.
-    intros.
-    simpl. rewrite (queue_morph bstate1 bstate2 c_morph).
-    assert (action_morphism bstate1 = action_morphism bstate1').
-    - apply functional_extensionality. intro a.
-        unfold action_morphism. f_equal.
-        destruct (act_body a); auto.
-        rewrite (contracts_eq bstate1 bstate1' env_equiv to). auto.
-    - rewrite <- H8. 
-        exact (permutation_preserved_over_map (action_morphism bstate1) (chain_state_queue bstate1) (chain_state_queue bstate1') H7).
-Qed.
-
-Lemma chainstate_morphism_new_env_equiv_permute 
-    (bstate1 bstate2 bstate1' : ChainState)
-    (e_morph : EnvironmentMorphism bstate1 bstate2) : 
-    let bstate2' := bstate_transform_step bstate1' in 
-    EnvironmentEquiv bstate1' bstate1 -> 
-    EnvironmentEquiv bstate2' bstate2.
-Proof.
-    intros bstate2' EE1.
-    exact 
-    (symmetry
-    (env_equiv_carries_over_env_morphism 
-        bstate1 bstate1' bstate2 bstate2' 
-        e_morph
-        (env_morph_step bstate1')
-        (symmetry EE1))).
-Qed.
-
-Lemma chainstate_morphism_new_queue_prev 
-    (bstate1 bstate2 : ChainState)
-    (c_morph : ChainStateMorphism bstate1 bstate2) : 
-    forall (act : Action) (acts : list Action),
-    chain_state_queue bstate1 = act :: acts -> 
-    let new_act := action_morphism bstate1 act in 
-    let new_acts := List.map (action_morphism bstate1) acts in
-    chain_state_queue bstate2 = new_act :: new_acts.
-Proof.
-    intros.
-    unfold new_act. unfold new_acts.
-    rewrite (queue_morph bstate1 bstate2 c_morph). 
-    rewrite H7.
-    auto.
-Qed.
-
-Lemma chainstate_morphism_new_act_eval_true 
-    (bstate1 bstate2 bstate1' : ChainState)
-    (c_morph : ChainStateMorphism bstate1 bstate2) : 
-    forall (act : Action) (new_acts : list Action),
-    let act' := action_morphism bstate1 act in 
-    let new_acts' := List.map (action_morphism bstate1) new_acts in 
-    let bstate2' := bstate_transform_step bstate1' in  
-    ActionEvaluation bstate1 act  bstate1' new_acts ->
-    ActionEvaluation bstate2 act' bstate2' new_acts'.
-Proof. Admitted.
-
-(* TODO transform bstate back *)
-Lemma act_eval_pullback 
-    (bstate1 bstate2 : ChainState) 
-    (c_morph : ChainStateMorphism bstate1 bstate2)
-    (bstate : Environment) (act : Action) (new_acts : list Action) : 
-    let act' := action_morphism bstate1 act in 
-    ActionEvaluation bstate2 act' bstate new_acts ->
-    ActionEvaluation bstate1 act  bstate new_acts.
-Proof. Admitted.
-
-Lemma chainstate_morphism_new_act_eval_false
-    (bstate1 bstate2 : ChainState) 
-    (c_morph : ChainStateMorphism bstate1 bstate2)
-    (act : Action) : 
-    let act' := action_morphism bstate1 act in 
-    (forall bstate new_acts, ActionEvaluation bstate1 act  bstate new_acts -> False) ->
-    (forall bstate new_acts, ActionEvaluation bstate2 act' bstate new_acts -> False).
-Proof.
-    intros.
-    apply (H7 bstate new_acts).
-    apply (act_eval_pullback bstate1 bstate2 c_morph bstate act new_acts).
-    exact X.
-Qed.
-
-Lemma list_map_concat {A B : Type} {g : A -> B} : 
-    forall (l1 l2 : list A), 
-    List.map g (l1 ++ l2) = (List.map g l1) ++ (List.map g l2).
-Proof.
-    intros. 
-    induction l1.
-    - auto.
-    - assert (((a :: l1) ++ l2) = a :: (l1 ++ l2)); auto. rewrite H7.
-        assert (forall a' k, map g (a' :: k) = (g a') :: map g k); auto. 
-        rewrite (H8 a (l1 ++ l2)).
-        rewrite (H8 a l1).
-        assert (forall (a':B) k1 k2, (a' :: k1) ++ k2 = a' :: (k1 ++ k2)); auto.
-        rewrite (H9 (g a) (map g l1) (map g l2)).
-        rewrite IHl1. reflexivity.
-Qed.
-
-Lemma chainstate_morphism_new_queue_next
-    (bstate1 bstate2 bstate1' : ChainState)
-    (c_morph : ChainStateMorphism bstate1 bstate2) : 
-    forall (new_acts : list Action) (acts : list Action),
-    chain_state_queue bstate1' = new_acts ++ acts -> 
-    let bstate2'  := bstate_transform_step bstate1' in  
-    let new_acts' := List.map (action_morphism bstate1) new_acts in 
-    let acts'     := List.map (action_morphism bstate1) acts in
-    chain_state_queue bstate2' = new_acts' ++ acts'.
-Proof.
-    intros.
-    unfold bstate2'.
-    unfold bstate_transform_step. simpl.
-    unfold new_acts'. unfold acts'. rewrite H7.
-    rewrite <- (list_map_concat new_acts acts).
-    (assert (action_morphism bstate1' = action_morphism bstate1)).
-    - apply functional_extensionality. intro x.
-        destruct x.
-        unfold action_morphism. simpl. f_equal.
-        destruct act_body; auto.
-        admit.
-    - rewrite H8. reflexivity.
-Admitted.
-
-Lemma chainstate_morphism_queue_next_action_invalid
-    (bstate1 bstate2 bstate1' : ChainState) 
-    (acts : list Action): 
-    let bstate2' := bstate_transform_step bstate1' in  
-    let acts' := List.map (action_morphism bstate1) acts in 
-    chain_state_queue bstate1' = acts ->
-    chain_state_queue bstate2' = acts'.
-Proof. Admitted.
-
-Lemma chainstate_morphism_from_acct
-    (bstate : ChainState) (act : Action) : 
-    act_is_from_account act -> 
-    act_is_from_account (action_morphism bstate act).
-Proof.
-    unfold act_is_from_account.
-    intros.
-    assert (act_from (action_morphism bstate act) = act_from act).
-    - unfold action_morphism. auto.
-    - rewrite H8. exact H7.
-Qed.
-
-Definition step_transform_step 
-    (bstate1 bstate2 bstate1' : ChainState)
-    (c_morph : ChainStateMorphism bstate1 bstate2) 
-    (step : ChainStep bstate1 bstate1') : 
-    let bstate2' := bstate_transform_step bstate1' in  
-    (ChainStep bstate2 bstate2') :=
-    let bstate2' := bstate_transform_step bstate1' in  
-    let c_morph' := chainstate_morphism_step bstate1' in 
-    match step with 
-    | step_block _ _ header prev_queue_empty next_block_valid no_acts_from_accounts origin_eq_from 
-        env_equiv  => 
-        (* modified header *)
-        let header' := header in 
-        (* modified prev_queue_empty *)
-        let prev_queue_empty' := 
-            chainstate_morphism_empty_queue bstate1 bstate2 c_morph prev_queue_empty in 
-        (* modified next_block_valid *)
-        let next_block_valid' := 
-            chainstate_morphism_next_block_valid bstate1 bstate2 c_morph header next_block_valid in 
-        (* modified no_acts_from_accounts *)
-        let no_acts_from_accounts' := 
-            chainstate_morphism_no_acts_from_accounts bstate1' no_acts_from_accounts in
-        (* modified origin_eq_from *)
-        let origin_eq_from' :=
-            chainstate_morphism_origin_eq_from bstate1' origin_eq_from in 
-        (* modified env_equiv *)
-        let env_equiv' :=
-            chainstate_morphism_new_env_equiv_add_block bstate1 bstate2 bstate1' 
-            (env_morph bstate1 bstate2 c_morph) header env_equiv in
-        (* the new step_block *)
-        step_block bstate2 bstate2'
-            header' prev_queue_empty' next_block_valid' no_acts_from_accounts' 
-            origin_eq_from' env_equiv'
-    | step_action _ _ act acts new_acts queue_prev act_eval_true queue_next => 
-        (* modified act *)
-        let act' := action_morphism bstate1 act in 
-        (* modified acts *)
-        let acts' := 
-            List.map (action_morphism bstate1) acts in 
-        (* modified new_acts *)
-        let new_acts' := 
-            List.map (action_morphism bstate1) new_acts in 
-        (* modified queue_prev *)
-        let queue_prev' := 
-            chainstate_morphism_new_queue_prev bstate1 bstate2 c_morph act acts queue_prev in 
-        (* modified act_eval_true *)
-        let act_eval_true' := 
-            chainstate_morphism_new_act_eval_true bstate1 bstate2 bstate1' c_morph act new_acts act_eval_true in 
-        (* modified queue_next *)
-        let queue_next' := 
-            chainstate_morphism_new_queue_next bstate1 bstate2 bstate1' c_morph new_acts acts queue_next in
-        (* the new step_block *)
-        step_action bstate2 bstate2' act' acts' new_acts' queue_prev' act_eval_true' queue_next'
-    | step_action_invalid _ _ act acts env_equiv queue_prev queue_next from_acct actn_eval_false => 
-        (* modified act *)
-        let act' := action_morphism bstate1 act in 
-        (* modified acts *)
-        let acts' := 
-            List.map (action_morphism bstate1) acts in 
-        (* modified env_equiv *)
-        let env_equiv' := 
-            chainstate_morphism_new_env_equiv_permute bstate1 bstate2 bstate1' 
-            (env_morph bstate1 bstate2 c_morph) env_equiv in 
-        (* modified queue_prev *)
-        let queue_prev' := 
-            chainstate_morphism_new_queue_prev bstate1 bstate2 c_morph act acts queue_prev in 
-        (* modified queue_next *)
-        let queue_next' := 
-            chainstate_morphism_queue_next_action_invalid bstate1 bstate2 bstate1' acts queue_next in 
-        (* modified from_acct *)
-        let from_acct' := 
-            chainstate_morphism_from_acct bstate1 act from_acct in 
-        (* modified actn_eval_false *)
-        let actn_eval_false' := 
-            chainstate_morphism_new_act_eval_false bstate1 bstate2 c_morph act actn_eval_false in 
-        (* the new step_block *)
-        step_action_invalid bstate2 bstate2' act' acts' env_equiv' queue_prev' queue_next' from_acct' actn_eval_false'
-    | step_permute _ _ env_equiv permuted => 
-        (* modified env_equiv *)
-        let env_equiv' := 
-            chainstate_morphism_new_env_equiv_permute bstate1 bstate2 bstate1' 
-            (env_morph bstate1 bstate2 c_morph) env_equiv in 
-        (* modified permutation *)
-        let permuted' := 
-            chainstate_morphism_new_permuted bstate1 bstate2 bstate1' (symmetry env_equiv) c_morph permuted in 
-        (* the new step_block *)
-        step_permute bstate2 bstate2' env_equiv' permuted' 
-    end.
-
-Lemma empty_chainstate_morphism : ChainStateMorphism empty_state empty_state. 
-Proof.
-    apply build_chainstate_morphism; auto.
-    apply build_env_morphism; auto.
-Qed.
-
-Definition caddr_implication_step (bstate1' : ChainState) (caddr : Address) :
-    let bstate2' := bstate_transform_step bstate1' in  
-    env_contracts bstate1' caddr = Some (C1 : WeakContract) -> 
-    env_contracts bstate2' caddr = Some (C2 : WeakContract).
-Proof.
-    intros. unfold bstate2'.
-    unfold bstate_transform_step. simpl.
-    rewrite H7. 
-    destruct (C1 =? C1)%wc; auto.
-    contradiction.
-Qed.
-    
-(* Theorem: A contract morphism can be lifted into a morphism of ChainStates *)
-Theorem cm_lift :
-    forall  bstate1 caddr (trace : ChainTrace empty_state bstate1),
-    exists  (* a new bstate related to the old *)
-            (bstate2 : ChainState) 
-            (bstate_morph : ChainStateMorphism bstate1 bstate2)
-            (* a new trace related to the old *)
-            (trace2 : ChainTrace empty_state bstate2),
-            (* with C2 swapped out for C1 *)
-            env_contracts bstate1 caddr = Some (C1 : WeakContract) -> 
-            env_contracts bstate2 caddr = Some (C2 : WeakContract).
-Proof.
-    (* we induct over the trace *)
-    intros.
-    remember empty_state eqn:genesis_empty. induction trace.
-    - rewrite genesis_empty. 
-        exists empty_state. exists empty_chainstate_morphism. 
-        exists ChainedList.clnil.
-        intro. assert (env_contracts empty_state caddr = None); auto. 
-        rewrite H8 in H7. congruence.
-    - apply IHtrace in genesis_empty. clear IHtrace.
-        (* destruct IHtrace1 as [bstate2 H']. auto. admit. *)
-        destruct genesis_empty as [bstate2 genesis_empty]. 
-        destruct genesis_empty as [bstate_morph genesis_empty]. 
-        destruct genesis_empty as [trace2 addr_implication].
-        (* construct the new bstate and trace *)
-        set (bstate2' := bstate_transform_step to).
-        set (l' := step_transform_step mid bstate2 to bstate_morph l).
-        set (trace2' := ChainedList.snoc trace2 l').
-        (* construct the relationships *)
-        set (bstate_morph' := chainstate_morphism_step to).
-        set (caddr_impl := caddr_implication_step to caddr).
-        exists bstate2'. 
-        exists bstate_morph'. 
-        exists trace2'.
-        exact caddr_impl.
-Qed.
-
-End ContractMorphismLift.
-
-Section ContractMorphismLiftCompose.
-
-(* Some results about the lifted morphism *)
-(*
-Lemma id_lifts_to_id 
-    { Setup Setup' Msg Msg' State State' Error Error' : Type }
-    `{Serializable Msg}  `{Serializable Setup}  `{Serializable State}  `{Serializable Error}
-    `{Serializable Msg'} `{Serializable Setup'} `{Serializable State'} `{Serializable Error'}
-    {C1 : Contract Setup Msg State Error} {C2 : Contract Setup' Msg' State' Error'} : todo "".
-Proof. exact (todo ""). Qed.
-
-Lemma morphisms_lift_compose
-    { Setup Setup' Msg Msg' State State' Error Error' : Type }
-    `{Serializable Msg}  `{Serializable Setup}  `{Serializable State}  `{Serializable Error}
-    `{Serializable Msg'} `{Serializable Setup'} `{Serializable State'} `{Serializable Error'}
-    {C1 : Contract Setup Msg State Error} {C2 : Contract Setup' Msg' State' Error'} : todo "".
-
-Lemma inj_lifts_to_inj
-    { Setup Setup' Msg Msg' State State' Error Error' : Type }
-    `{Serializable Msg}  `{Serializable Setup}  `{Serializable State}  `{Serializable Error}
-    `{Serializable Msg'} `{Serializable Setup'} `{Serializable State'} `{Serializable Error'}
-    {C1 : Contract Setup Msg State Error} {C2 : Contract Setup' Msg' State' Error'} : todo "".
-
-Lemma surj_lifts_to_surj
-    { Setup Setup' Msg Msg' State State' Error Error' : Type }
-    `{Serializable Msg}  `{Serializable Setup}  `{Serializable State}  `{Serializable Error}
-    `{Serializable Msg'} `{Serializable Setup'} `{Serializable State'} `{Serializable Error'}
-    {C1 : Contract Setup Msg State Error} {C2 : Contract Setup' Msg' State' Error'} : todo "".
-*)
-
-End ContractMorphismLiftCompose.
-
-
+(** We will treat various type of contract morphisms, starting with isomorphisms. *)
 Section Isomorphisms.
 
 Definition is_iso {A B : Type} (f : A -> B) (g : B -> A) : Prop := 
@@ -1168,7 +479,7 @@ Proof.
         destruct iso_r_inputs as [iso_r_inputs1 iso_r_inputs2].
         destruct iso_r_outputs as [iso_r_outputs1 iso_r_outputs2].
         unfold is_iso_cm. unfold composition_cm. unfold id_cm. 
-        unfold id_cm_init. unfold id_cm_recv. unfold id_morph. 
+        unfold id_cm_init. unfold id_cm_recv. unfold id_fun. 
         split.
         +   apply is_eq_cm.
             * apply is_eq_cm_init; simpl.
@@ -1185,7 +496,7 @@ Proof.
                 ** exact iso_r_inputs2.
                 ** exact iso_r_outputs2. 
     -   unfold is_iso_cm. unfold composition_cm.  unfold id_cm. 
-        unfold id_cm_init. unfold id_cm_recv. unfold id_morph.
+        unfold id_cm_init. unfold id_cm_recv. unfold id_fun.
         intro is_iso_H. destruct is_iso_H as [is_iso_H1 is_iso_H2].
         inversion is_iso_H1. inversion is_iso_H2.
         auto.
@@ -1243,187 +554,12 @@ Proof.
         rewrite iso_f2. rewrite (composition_id_cm_right g). exact iso_g2.
 Qed.
 
-
-(*  Results about isomorphisms 
-
-    The following results show that :
-
-    (1) deploying isomorphic contracts produces isomorphic environments, or a bisimulation of 
-        environments
-    (2) an equivalence of environments is preserved under ActionEvaluation, where equivalent actions 
-        are paired via the isomorphism of environments
-
-    Together, these results show that deploying isomorphic contracts results two separate chains, along with a bisimulation of chains. Functionally, then, the chains behave in equivalent ways.
-*)
-
-Definition weak_contracts_isomorphic (W1 W2 : option WeakContract) : Prop := todo "".
-Definition serialized_state_isomorphic (s1 s2 : option SerializedValue) : Prop := todo "".
-
-(* we define a (functional) equivalence of environments via a function : this is a bisimulation *)
-Record EnvironmentBisimulation (e1 e2 : Environment) : Prop := {
-    chain_eq : env_chain e1 = env_chain e2 ; 
-    account_balances_eq :
-        forall a, env_account_balances e1 a = env_account_balances e2 a;
-    contracts_eq :
-        forall a, weak_contracts_isomorphic (env_contracts e1 a) (env_contracts e2 a);
-    contract_states_eq :
-        forall a, serialized_state_isomorphic (env_contract_states e1 a) (env_contract_states e2 a);
-}.
-    
-(* should rely on environment bisimulation *)
-Record ChainStateBisimulation (b1 b2 : ChainState) : Prop := {
-    env_eq' : EnvironmentBisimulation b1 b2 ; 
-    queue_eq' : chain_state_queue b1 = chain_state_queue b2 ;
-}.
-
-(* every environment is a bisimulation of itself *)
-Lemma env_equiv_then_bisimulation:
-    forall e1 e2,
-    EnvironmentEquiv e1 e2 -> 
-    EnvironmentBisimulation e1 e2.
-Proof. Admitted.
-
-(* deploying isomorphic contracts preserves a bisimulation *)
-Definition isomorphic_contracts_to_bisimulation
-        { Setup Setup' Msg Msg' State State' Error Error' : Type }
-        `{Serializable Msg}  `{Serializable Setup}  `{Serializable State}  `{Serializable Error}
-        `{Serializable Msg'} `{Serializable Setup'} `{Serializable State'} `{Serializable Error'}
-        {C : Contract Setup Msg State Error} {C' : Contract Setup' Msg' State' Error'} : 
-    contracts_isomorphic C C' ->
-    (* start with equivalent, reachable environments *)
-    forall env1 env2, 
-    reachable env1 ->
-    reachable env2 ->
-    EnvironmentBisimulation env1 env2 -> 
-    forall env1' env2' act_deploy_C act_deploy_C' new_acts s s' amt,
-    (* the environment we get by deploying C  *)
-    ActionEvaluation env1 act_deploy_C env1' new_acts -> 
-        act_deploy_C.(act_body) = act_deploy amt C s ->
-    (* the environment we get by deploying C'  *)
-    ActionEvaluation env2 act_deploy_C' env2' new_acts -> 
-        act_deploy_C'.(act_body) = act_deploy amt C' s' ->
-    (* the setups are equivalent under the isomorphism *)
-    s = s' -> (* TODO *)
-    (* they are deployed to the same address *)
-    forall caddr caddr',
-        env_contracts env1'  caddr  = Some (C  : WeakContract) -> 
-        env_contracts env2' caddr' = Some (C' : WeakContract) ->
-        caddr = caddr' ->
-    (* they are deployed BY the same address (and origin) *)
-    act_deploy_C.(act_from) = act_deploy_C'.(act_from) ->
-    act_deploy_C.(act_origin) = act_deploy_C'.(act_origin) ->
-    (* the isomorphisms f and g lift to a bisimulation of env' and env'' *)
-    EnvironmentBisimulation env1' env2'
-    := todo "".
-
-(* if C and C' are isomorphic, then deploying  *)
-(* base case *)
-Lemma iso_cm_then_iso_env_init 
-        { Setup Setup' Msg Msg' State State' Error Error' : Type }
-        `{Serializable Msg}  `{Serializable Setup}  `{Serializable State}  `{Serializable Error}
-        `{Serializable Msg'} `{Serializable Setup'} `{Serializable State'} `{Serializable Error'}
-        {C : Contract Setup Msg State Error} {C' : Contract Setup' Msg' State' Error'} : 
-    forall (f : ContractMorphism C C') (g : ContractMorphism C' C),
-    is_iso_cm f g -> 
-    (* for all reachable states *)
-    forall env, reachable env -> 
-    forall env' env'' act_deploy_C act_deploy_C' new_acts s amt,
-    (* the environment we get by deploying C  *)
-    ActionEvaluation env act_deploy_C  env'  new_acts -> 
-        act_deploy_C.(act_body)  = act_deploy amt C  s ->
-    (* the environment we get by deploying C'  *)
-    ActionEvaluation env act_deploy_C' env'' new_acts -> 
-        act_deploy_C'.(act_body) = act_deploy amt C' s ->
-    (* they are deployed to the same address *)
-    forall caddr caddr',
-        env_contracts env'  caddr  = Some (C  : WeakContract) -> 
-        env_contracts env'' caddr' = Some (C' : WeakContract) ->
-        caddr = caddr' ->
-    (* they are deployed BY the same address (and origin) *)
-    act_deploy_C.(act_from) = act_deploy_C'.(act_from) ->
-    act_deploy_C.(act_origin) = act_deploy_C'.(act_origin) ->
-    (* the two environments are equivalent *)
-    EnvironmentBisimulation env' env''.
-Proof. Admitted.
-(* get a witness that env bisimulates itself, apply function above *)
-
-(* inductive step *)
-Lemma iso_cm_then_iso_env_recv : 
-    forall bstate1  bstate2,  EnvironmentBisimulation bstate1 bstate2 -> 
-    forall bstate1' bstate2' act1 act2 new_acts,
-        ActionEvaluation bstate1 act1 bstate1' new_acts -> 
-        ActionEvaluation bstate2 act2 bstate2' new_acts -> 
-        (* the act should be equivalent, not identical *)
-        act1 = act2 -> (* TODO *)
-        EnvironmentBisimulation bstate1' bstate2'.
-Proof. Admitted.
-
-(* Main result for isomorphisms *)
-Theorem iso_cm_then_iso_bstate
-        { Setup Setup' Msg Msg' State State' Error Error' : Type }
-        `{Serializable Msg}  `{Serializable Setup}  `{Serializable State}  `{Serializable Error}
-        `{Serializable Msg'} `{Serializable Setup'} `{Serializable State'} `{Serializable Error'}
-        {C1 : Contract Setup Msg State Error} {C2 : Contract Setup' Msg' State' Error'} : 
-    forall (f : ContractMorphism C1 C2) (g : ContractMorphism C2 C1),
-    is_iso_cm f g -> 
-    (* for all reachable states *)
-    forall bstate, reachable bstate -> 
-    forall bstate1 bstate2 (* the new blockchain states *)
-           acts new_acts s amt (* queued actions, actions emitted by C1 and C2, setup, and amt *)
-           act_deploy_C1 act_deploy_C2 (* the actions of deploying C1 and C2 *)
-           actneval1 actneval2 (* the inhabitants of ActionEvaluation *)
-           state_queue1 state_queue1' (* proof that the state queues evolve correctly *)
-           state_queue2 state_queue2'
-           cstep1 cstep2, (* the chainstep *)
-    (* the bstate we get by deploying C  *)
-    cstep1 = step_action bstate bstate1 act_deploy_C1 acts new_acts state_queue1 actneval1 state_queue1' -> 
-    act_deploy_C1.(act_body) = act_deploy amt C1  s ->
-    (* the bstate we get by deploying C'  *)
-    cstep2 = step_action bstate bstate2 act_deploy_C2 acts new_acts state_queue2 actneval2 state_queue2' -> 
-    act_deploy_C2.(act_body) = act_deploy amt C2 s ->
-    (* they are deployed to the same address *)
-    forall caddr1 caddr2,
-        env_contracts bstate1 caddr1 = Some (C1 : WeakContract) -> 
-        env_contracts bstate2 caddr2 = Some (C2 : WeakContract) ->
-        caddr1 = caddr2 ->
-    (* they are deployed BY the same address (and origin) *)
-    act_deploy_C1.(act_from)   = act_deploy_C2.(act_from) ->
-    act_deploy_C1.(act_origin) = act_deploy_C2.(act_origin) ->
-    (* for any state reachable through env1, we have a corresponding isomorphic state reachable through env2 *)
-    forall bstate1', reachable_through bstate1 bstate1' -> 
-    exists bstate2', 
-        reachable_through bstate2 bstate2' /\
-        ChainStateBisimulation bstate1' bstate2'.
-Proof. Admitted.
-
-
-(* for any reachable state with C1 deployed, we have an isomorphic reachable state with C2 deployed at the same address *)
-Definition iso_trace bstate bstate1 bstate2 :
-    ChainTrace bstate bstate1 -> ChainTrace bstate bstate2 := todo "".
-
-Definition iso_bstate (bstate1 bstate2 : ChainState) : Prop := todo "".
-
-Theorem iso_cm_then_iso_bstate2 
-        { Setup Setup' Msg Msg' State State' Error Error' : Type }
-        `{Serializable Msg}  `{Serializable Setup}  `{Serializable State}  `{Serializable Error}
-        `{Serializable Msg'} `{Serializable Setup'} `{Serializable State'} `{Serializable Error'}
-        {C1 : Contract Setup Msg State Error} {C2 : Contract Setup' Msg' State' Error'} : 
-    contracts_isomorphic C1 C2 -> 
-    (* forall reachable states *)
-    forall bstate1 caddr (trace1 : ChainTrace empty_state bstate1), 
-    reachable bstate1 -> 
-    env_contracts bstate1 caddr = Some (C1 : WeakContract) -> 
-    (* we can produce an isomorphic trace *)
-    exists (bstate2 : ChainState) (trace2 : ChainTrace empty_state bstate2),
-    env_contracts bstate2 caddr = Some (C2 : WeakContract) /\ 
-    iso_bstate bstate1 bstate2 /\ (* todo : perhaps produce the isomorphism *)
-    trace2 = iso_trace empty_state bstate1 bstate2 trace1.
-Proof. Admitted.
-
 End Isomorphisms.
 
 
-Section Monomorphisms.
+(** Now, onto injections *)
+Section Injections.
+
 Definition is_inj {A B : Type} (f : A -> B) : Prop := 
     forall (a a' : A), f a = f a' -> a = a'.
 
@@ -1447,34 +583,11 @@ Definition contract_embeds
         (C1 : Contract Setup Msg State Error) (C2 : Contract Setup' Msg' State' Error') := 
     exists (f : ContractMorphism C1 C2), is_inj_cm f.
 
-(* results about monomorphisms *)
-(* an EMBEDDING of traces *)
-
-Definition embed_trace bstate bstate1 bstate2 :
-    ChainTrace bstate bstate1 -> ChainTrace bstate bstate2 := todo "".
-Definition bstate_embeds (bstate1 bstate2 : ChainState) : Prop := todo "".
-
-Theorem inj_cm_then_trace_embedding 
-        { Setup Setup' Msg Msg' State State' Error Error' : Type }
-        `{Serializable Msg}  `{Serializable Setup}  `{Serializable State}  `{Serializable Error}
-        `{Serializable Msg'} `{Serializable Setup'} `{Serializable State'} `{Serializable Error'}
-        {C1 : Contract Setup Msg State Error} {C2 : Contract Setup' Msg' State' Error'} : 
-    contract_embeds C1 C2 -> 
-    (* for all reachable states where C1 is deployed *)
-    forall bstate1 caddr (trace1 : ChainTrace empty_state bstate1),
-    reachable bstate1 -> 
-    env_contracts bstate1 caddr = Some (C1 : WeakContract) ->
-    (* we can produce a trace in the case that C2 was deployed rather than C1 *)
-    exists (bstate2 : ChainState) (trace2 : ChainTrace empty_state bstate2),
-    env_contracts bstate2 caddr = Some (C2 : WeakContract) /\ 
-    bstate_embeds bstate1 bstate2 /\ (* exists an embedding morphism *)
-    trace2 = embed_trace empty_state bstate1 bstate2 trace1. (* we can construct a trace to reachable bstate2 *)
-Proof. Admitted.    
-
-End Monomorphisms.
+End Injections.
 
 
-Section Epimorphisms.
+(** Finally, we treat surjections, or quotients *)
+Section Surjections.
 
 Definition is_surj {A B : Type} (f : A -> B) : Prop := 
     forall (b : B), exists (a : A), f a = b.
@@ -1492,9 +605,6 @@ Definition is_surj_cm
     is_surj (recv_inputs C C' (recv_cm f)) /\
     is_surj (recv_outputs C C' (recv_cm f)).
 
-(* TODO : Result about surjections : possibly about retracts, splitting C into C + C' via a retract *)
-(*                                 : possibly about upgradeability too *)
-
 Definition contract_surjects 
         { Setup Setup' Msg Msg' State State' Error Error' : Type }
         `{Serializable Msg}  `{Serializable Setup}  `{Serializable State}  `{Serializable Error}
@@ -1502,29 +612,11 @@ Definition contract_surjects
         (C1 : Contract Setup Msg State Error) (C2 : Contract Setup' Msg' State' Error') := 
     exists (f : ContractMorphism C1 C2), is_surj_cm f.
 
-Definition bstate_surjects (bstate1 bstate2 : ChainState) : Prop := todo "".
-Definition quotient_trace bstate bstate1 bstate2 :
-    ChainTrace bstate bstate1 -> ChainTrace bstate bstate2 := todo "".
-
-Theorem surj_cm_surj_bstate
-        { Setup Setup' Msg Msg' State State' Error Error' : Type }
-        `{Serializable Msg}  `{Serializable Setup}  `{Serializable State}  `{Serializable Error}
-        `{Serializable Msg'} `{Serializable Setup'} `{Serializable State'} `{Serializable Error'}
-        {C1 : Contract Setup Msg State Error} {C2 : Contract Setup' Msg' State' Error'} : 
-    contract_surjects C1 C2 -> 
-    (* for all reachable states where C1 is deployed *)
-    forall bstate1 caddr (trace1 : ChainTrace empty_state bstate1),
-    env_contracts bstate1 caddr = Some (C1 : WeakContract) ->
-    (* we can produce a trace in the case that C2 was deployed rather than C1 *)
-    exists (bstate2 : ChainState) (trace2 : ChainTrace empty_state bstate2),
-    env_contracts bstate2 caddr = Some (C2 : WeakContract) /\ 
-    bstate_surjects bstate1 bstate2 /\ (* exists a surjection morphism *)
-    trace2 = quotient_trace empty_state bstate1 bstate2 trace1. (* we can compress trace1 into trace2 *)
-Proof. Admitted.
-
-End Epimorphisms.
+End Surjections.
 
 
+(** We have some interesting categorical properties, including the existence of a terminal
+    contract. (Note that we have not yet proved uniqueness of the terminal morphism.) *)
 Section TerminalContract.
     Import ListNotations.
     Set Nonrecursive Elimination Schemes.
@@ -1638,17 +730,904 @@ Definition null_morphism : ContractMorphism C null_contract :=
         cm_recv := morph_recv ;
     |}.
 
-(* TODO: this is more nuanced 
-Lemma null_morphism_unique : forall (f : ContractMorphism C null_contract), f = null_morphism.
-Proof. 
-    intro. apply is_eq_cm; try apply is_eq_cm_init; try apply is_eq_cm_recv; apply functional_extensionality; intro.
-    -   destruct x as [x' s]. destruct x' as [c ctx].
-        admit.
-    -   destruct x. Admitted.*)
+(* TODO: Prove uniqueness *)
 
 End TerminalContract.
 
 
+(** The definition of contract morphisms is fairly general, and 
+    somewhat difficult to work with. As we proceed, we will use 
+    simple contract morphisms, which can be decomposed as functions 
+    between state, msg, setup, and error types along with the corresponding
+    coherence result.
+    
+    This simpler structure will allow us to lift contract morphisms into
+    a transformation of chainstate and trace.
+    
+    Note that these simpler morphisms do not modify balances or emitted 
+    actions. Future work could include generalizing the lifting result
+    to allow for more contract morphisms.
+*)
+Section SimpleContractMorphism.
 
+(** Some auxiliary functions for transforming component functions into morphism form *)
+Definition init_result_transform 
+        { State State' Error Error' : Type }
+    (state_morph : State -> State')
+    (error_morph : Error -> Error')
+    (x : result State Error) : result State' Error' :=
+    match x with 
+    | Ok t => Ok (state_morph t)
+    | Err e => Err (error_morph e)
+    end.
+
+Definition recv_result_transform 
+        { State State' Error Error' : Type }
+    (state_morph : State -> State')
+    (error_morph : Error -> Error')
+    (x : result (State  * list ActionBody) Error) : result (State' * list ActionBody) Error' := 
+        match x with 
+        | Ok t => let '(st, l) := t in Ok (state_morph st, l)
+        | Err e => Err (error_morph e)
+        end.
+
+(** We explicitly construct the components *)
+(* the init component *)
+Lemma init_commutes_simple 
+    { Setup Setup' Msg Msg' State State' Error Error' : Type }
+    `{Serializable Msg}  `{Serializable Setup}  `{Serializable State}  `{Serializable Error}
+    `{Serializable Msg'} `{Serializable Setup'} `{Serializable State'} `{Serializable Error'}
+    {C1 : Contract Setup Msg State Error} 
+    {C2 : Contract Setup' Msg' State' Error'}
+    (* the components of f *)
+    (setup_morph : Setup -> Setup')
+    (state_morph : State -> State')
+    (error_morph : Error -> Error')
+    (* coherence conditions *)
+    (init_coherence : forall c ctx s, 
+        (init_result_transform state_morph error_morph) ((init C1) c ctx s) = (init C2) c ctx (setup_morph s)) : 
+    init_morphs_commute 
+        C1.(init) C2.(init)
+        (fun (x : Chain * ContractCallContext * Setup) => 
+            let '(c, ctx, s) := x in (c, ctx, setup_morph s))
+        (init_result_transform state_morph error_morph).
+Proof.
+    unfold init_morphs_commute. 
+    intro. destruct x. destruct p.
+    unfold uncurry_fun3. simpl.
+    rewrite <- (init_coherence c c0 s).
+    unfold init_outputs. 
+    reflexivity.
+Qed.
+
+Definition simple_cm_init 
+    { Setup Setup' Msg Msg' State State' Error Error' : Type }
+    `{Serializable Msg}  `{Serializable Setup}  `{Serializable State}  `{Serializable Error}
+    `{Serializable Msg'} `{Serializable Setup'} `{Serializable State'} `{Serializable Error'}
+    {C1 : Contract Setup Msg State Error} 
+    {C2 : Contract Setup' Msg' State' Error'}
+    (* the components of f *)
+    (setup_morph : Setup -> Setup')
+    (state_morph : State -> State')
+    (error_morph : Error -> Error')
+    (* coherence conditions *)
+    (init_coherence : forall c ctx s, 
+        (init_result_transform state_morph error_morph) ((init C1) c ctx s) = (init C2) c ctx (setup_morph s)) : 
+    InitCM C1 C2 := {| 
+        init_inputs := (fun (x : Chain * ContractCallContext * Setup) => 
+        let '(c, ctx, s) := x in (c, ctx, setup_morph s)) ; 
+        init_outputs := (init_result_transform state_morph error_morph) ; 
+        init_commutes := init_commutes_simple setup_morph state_morph error_morph init_coherence ;
+    |}.
+
+(* the recv component *)
+Lemma recv_commutes_simple 
+    { Setup Setup' Msg Msg' State State' Error Error' : Type }
+    `{Serializable Msg}  `{Serializable Setup}  `{Serializable State}  `{Serializable Error}
+    `{Serializable Msg'} `{Serializable Setup'} `{Serializable State'} `{Serializable Error'}
+    {C1 : Contract Setup Msg State Error} 
+    {C2 : Contract Setup' Msg' State' Error'}
+    (* the components of f *)
+    (msg_morph   : Msg   -> Msg')
+    (state_morph : State -> State')
+    (error_morph : Error -> Error')
+    (* coherence conditions *)
+    (recv_coherence : forall c ctx st op_msg, 
+        (recv_result_transform state_morph error_morph) ((receive C1) c ctx st op_msg) = 
+        (receive C2) c ctx (state_morph st) (option_fun msg_morph op_msg)) : 
+    recv_morphs_commute
+        C1.(receive) C2.(receive)
+        (fun (x : Chain * ContractCallContext * State * option Msg) => 
+            let '(c, ctx, st, op_msg) := x in (c, ctx, state_morph st, option_fun msg_morph op_msg))
+        (recv_result_transform state_morph error_morph).
+Proof.
+    unfold recv_morphs_commute. 
+    intro. destruct x. repeat destruct p.
+    unfold uncurry_fun4. simpl.
+    rewrite <- (recv_coherence c c0 s o).
+    unfold recv_outputs.
+    reflexivity.
+Qed.
+
+Definition simple_cm_recv 
+    { Setup Setup' Msg Msg' State State' Error Error' : Type }
+    `{Serializable Msg}  `{Serializable Setup}  `{Serializable State}  `{Serializable Error}
+    `{Serializable Msg'} `{Serializable Setup'} `{Serializable State'} `{Serializable Error'}
+    {C1 : Contract Setup Msg State Error} 
+    {C2 : Contract Setup' Msg' State' Error'}
+    (* the components of f *)
+    (msg_morph   : Msg   -> Msg')
+    (state_morph : State -> State')
+    (error_morph : Error -> Error')
+    (* coherence conditions *)
+    (recv_coherence : forall c ctx st op_msg, 
+        (recv_result_transform state_morph error_morph) ((receive C1) c ctx st op_msg) = 
+        (receive C2) c ctx (state_morph st) (option_fun msg_morph op_msg)) : 
+    RecvCM C1 C2 := {| 
+        recv_inputs := 
+            (fun (x : Chain * ContractCallContext * State * option Msg) => 
+                let '(c, ctx, st, op_msg) := x in (c, ctx, state_morph st, option_fun msg_morph op_msg)) ; 
+        recv_outputs := 
+            (recv_result_transform state_morph error_morph) ; 
+        recv_commutes := recv_commutes_simple msg_morph state_morph error_morph recv_coherence ;
+    |}.
+
+(* the simple contract morphism *)
+Definition simple_cm 
+    { Setup Setup' Msg Msg' State State' Error Error' : Type }
+    `{Serializable Msg}  `{Serializable Setup}  `{Serializable State}  `{Serializable Error}
+    `{Serializable Msg'} `{Serializable Setup'} `{Serializable State'} `{Serializable Error'}
+    {C1 : Contract Setup Msg State Error} 
+    {C2 : Contract Setup' Msg' State' Error'}
+    (* the components of f *)
+    (msg_morph   : Msg   -> Msg')
+    (setup_morph : Setup -> Setup')
+    (state_morph : State -> State')
+    (error_morph : Error -> Error')
+    (* coherence conditions *)
+    (init_coherence : forall c ctx s, 
+        (init_result_transform state_morph error_morph) ((init C1) c ctx s) = (init C2) c ctx (setup_morph s))
+    (recv_coherence : forall c ctx st op_msg, 
+        (recv_result_transform state_morph error_morph) ((receive C1) c ctx st op_msg) = 
+        (receive C2) c ctx (state_morph st) (option_fun msg_morph op_msg)) : 
+    ContractMorphism C1 C2 := {| 
+        cm_init := simple_cm_init setup_morph state_morph error_morph init_coherence ;
+        cm_recv := simple_cm_recv msg_morph   state_morph error_morph recv_coherence ;
+    |}.
+
+End SimpleContractMorphism.
+
+
+(** In this Section, we lift a contract morphism f to a transformation of bstate and trace.
+    The main result, cm_lift, is proved by induction over the trace.
+        The section is organized as follows:
+        1. Section ChainStateMorphism: 
+            - We define a morphism of environments and chainstates, parameterized by f
+            - We define the trivial morphism on trivial chainstates
+        1. Section BStateTransform:
+            - We define a transformation of bstate over f, bstate_transform_step, along with
+              a chainstate morphism from a state bstate to (bstate_transform_step bstate).
+            - This is done in chainstate_morphism_step.
+        2. Section CMLiftInductiveStep:
+            - We prove various lemmas for the inductive step of our proof. Each of these
+              has the prefix chainstep_transform_
+            - The inductive step is proved in the results chainstep_transform_step and 
+              caddr_implication_step
+        5. Finally, we prove the main result cm_lift
+*)
+Section ContractMorphismLift.
+Context 
+    (* we can lift a morphism of contracts, parameterized by the morphpism f and the address of C1 *)
+    { Setup Setup' Msg Msg' State State' Error Error' : Type }
+    `{Serializable Msg}  `{Serializable Setup}  `{Serializable State}  `{Serializable Error}
+    `{Serializable Msg'} `{Serializable Setup'} `{Serializable State'} `{Serializable Error'}
+    {C1 : Contract Setup Msg State Error} {C2 : Contract Setup' Msg' State' Error'}
+    {f : ContractMorphism C1 C2}.
+
+Variable 
+    (* f must be decomposable as follows *)
+    (msg_morph   : Msg   -> Msg')
+    (setup_morph : Setup -> Setup')
+    (state_morph : State -> State')
+    (error_morph : Error -> Error')
+    (* with coherence conditions satisfied *)
+    (init_coherence : forall c ctx s, 
+        (init_result_transform state_morph error_morph) ((init C1) c ctx s) = (init C2) c ctx (setup_morph s))
+    (recv_coherence : forall c ctx st op_msg, 
+        (recv_result_transform state_morph error_morph) ((receive C1) c ctx st op_msg) = 
+        (receive C2) c ctx (state_morph st) (option_fun msg_morph op_msg))
+    (* f is decomposable *)
+    (f_decomposable : 
+        f = simple_cm msg_morph setup_morph state_morph error_morph init_coherence recv_coherence).
+
+(* TODO *)
+Definition wc_dec_eq : forall w1 w2 : WeakContract, {w1 = w2} + {w1 <> w1} := todo "".
+Declare Scope wc_scope.
+Delimit Scope wc_scope with wc.
+Bind Scope wc_scope with WeakContract.
+Infix "=?" := wc_dec_eq (at level 70) : wc_scope.
+
+Section ChainStateMorphism.
+(* Given f, we can transform actions *)
+Definition action_transform (native_env : Environment) (a : Action) : Action := {| 
+    act_origin := act_origin a ;
+    act_from := act_from a ;
+    act_body := 
+        match act_body a with 
+        (* contract calls into C1 change to calls into C2 *)
+        | act_call to amt msg => 
+            match env_contracts native_env to with 
+            | Some wc => 
+                if (wc =? contract_to_weak_contract C1)%wc
+                then act_call to amt (serialize_function msg_morph msg)
+                else act_body a
+            | None => act_body a
+            end
+        (* we deploy C2 instead of C1 *)
+        | act_deploy amt c setup => 
+            if (c =? contract_to_weak_contract C1)%wc
+            then act_deploy amt (contract_to_weak_contract C2) (serialize_function setup_morph setup)
+            else act_body a
+        (* all amounts stay the same, so we do not change transfers *)
+        | act_transfer _ _ => act_body a 
+        end
+|}.
+
+(* A morphism of Environments, parameterized implicitly over f by swapping out C2 for C1 *)
+Record EnvironmentMorphism (e1 e2 : Environment) := 
+    build_env_morphism {
+        chain_eq' : env_chain e1 = env_chain e2 ;
+        account_balances_eq' :
+            forall a, env_account_balances e1 a = env_account_balances e2 a ;
+        contracts_morph :
+            forall a, 
+                env_contracts e2 a = 
+                match env_contracts e1 a with 
+                | Some wc => 
+                    if (wc =? contract_to_weak_contract C1)%wc 
+                    then Some (contract_to_weak_contract C2) 
+                    else Some wc
+                | None => None 
+                end ;
+        contract_states_morph : 
+            forall a, 
+                env_contract_states e2 a = 
+                match env_contracts e1 a with 
+                | Some wc => 
+                    if (wc =? contract_to_weak_contract C1)%wc 
+                    then (option_fun (serialize_function state_morph)) (env_contract_states e1 a)
+                    else env_contract_states e1 a
+                | None => env_contract_states e1 a
+                end ;
+}.
+
+(* A morphism of ChainStates, parameterized implicitly over f *)
+Record ChainStateMorphism (cstate1 cstate2 : ChainState) := 
+    build_chainstate_morphism {
+        env_morph   : EnvironmentMorphism cstate1 cstate2 ;
+        queue_morph : chain_state_queue cstate2 = 
+                      List.map (action_transform cstate1) (chain_state_queue cstate1) ;
+    }.
+
+Lemma empty_chainstate_morphism : ChainStateMorphism empty_state empty_state. 
+Proof.
+    apply build_chainstate_morphism; auto.
+    apply build_env_morphism; auto.
+Qed.
+
+End ChainStateMorphism.
+
+
+Section BStateTransform.
+(* given a bstate, construct one over f that will (trivially) yield a ChainStateMorphism *)
+Definition bstate_transform_step (bstate : ChainState) : ChainState := 
+        let env := {| 
+            (* the same as bstate *)
+            env_chain := env_chain bstate ; 
+            (* the same as bstate *)
+            env_account_balances := env_account_balances bstate ; 
+            (* the contracts are transformed via the contract morphism *)
+            env_contracts := fun a =>
+                match env_contracts bstate a with 
+                | Some wc => 
+                    if (wc =? contract_to_weak_contract C1)%wc 
+                    then Some (contract_to_weak_contract C2)
+                    else Some wc 
+                | None => None
+                end ;
+            (* the contract states are transformed via the contract morphism *)
+            env_contract_states := fun a => 
+                match env_contracts bstate a with 
+                | Some wc => 
+                    if (wc =? contract_to_weak_contract C1)%wc 
+                    then (option_fun (serialize_function state_morph)) (env_contract_states bstate a)
+                    else env_contract_states bstate a
+                | None => env_contract_states bstate a
+                end ;
+        |} in
+        (* we just use the queue again from bstate1' *)
+        let queue := List.map (action_transform bstate) (chain_state_queue bstate) in 
+        (* return the new cstate *)
+        {| chain_state_env := env ; chain_state_queue := queue ; |}.
+
+(* Some lemmas to construct something in ChainStateMorphism bstate (bstate_transform_step bstate) *)
+Lemma env_morph_step_chain_eq (bstate1 : ChainState) : 
+        let bstate2 := bstate_transform_step bstate1 in
+        env_chain bstate1 = env_chain bstate2.
+Proof. auto. Qed.
+
+Definition env_morph_step_balances (bstate1 : ChainState) : 
+    let bstate2 := bstate_transform_step bstate1 in
+    forall a, env_account_balances bstate1 a = env_account_balances bstate2 a.
+Proof. auto. Qed.
+
+Definition env_morph_step_contracts (bstate1 : ChainState) :  
+    let bstate2 := bstate_transform_step bstate1 in
+    forall a, 
+        env_contracts bstate2 a = 
+        match env_contracts bstate1 a with 
+        | Some wc => 
+            if (wc =? contract_to_weak_contract C1)%wc 
+            then Some (contract_to_weak_contract C2) 
+            else Some wc
+        | None => None 
+        end.
+Proof. 
+    intros. 
+    unfold bstate2.
+    unfold bstate_transform_step. 
+    simpl. reflexivity.
+Qed.
+
+Definition env_morph_step_states (bstate1 : ChainState) : 
+    let bstate2 := bstate_transform_step bstate1 in
+    forall a,
+        env_contract_states bstate2 a = 
+        match env_contracts bstate1 a with 
+        | Some wc => 
+            if (wc =? contract_to_weak_contract C1)%wc 
+            then (option_fun (serialize_function state_morph)) (env_contract_states bstate1 a)
+            else env_contract_states bstate1 a
+        | None => env_contract_states bstate1 a
+        end.
+Proof.
+    intros.
+    unfold bstate2.
+    unfold bstate_transform_step.
+    simpl. reflexivity.
+Qed.
+
+Definition env_morph_step (bstate1 : ChainState) : 
+    let bstate2 := bstate_transform_step bstate1 in
+    EnvironmentMorphism bstate1 bstate2 := {| 
+        chain_eq' := env_morph_step_chain_eq bstate1 ; 
+        account_balances_eq' := env_morph_step_balances bstate1 ; 
+        contracts_morph := env_morph_step_contracts bstate1 ; 
+        contract_states_morph := env_morph_step_states bstate1 ;
+    |}.    
+
+Lemma queue_morphism_step (bstate1 : ChainState) : 
+    let bstate2 := bstate_transform_step bstate1 in  
+    chain_state_queue bstate2
+    = List.map (action_transform bstate1) (chain_state_queue bstate1).
+Proof. auto. Qed.
+
+(* We have ChainStateMorphism bstate (bstate_transform_step bstate) *)
+Definition chainstate_morphism_step (bstate1' : ChainState) : 
+    let bstate2' := bstate_transform_step bstate1' in  
+    (ChainStateMorphism bstate1' bstate2') := {|  
+        env_morph   := env_morph_step bstate1' ; 
+        queue_morph := queue_morphism_step bstate1' |}.
+
+End BStateTransform.
+
+
+Section CMLiftInductiveStep.
+(* the main result of this section is chainstep_transform_step, for which we need 
+   several lemmas, each of which are prefixed with chainstep_transform_ *)
+
+(* construct the step from bstate2 to bstate2' *)
+Lemma chainstep_transform_empty_queue 
+    (cstate1 cstate2 : ChainState) 
+    (m : ChainStateMorphism cstate1 cstate2) : 
+    chain_state_queue cstate1 = nil -> chain_state_queue cstate2 = nil.
+Proof. 
+    intro. rewrite (queue_morph cstate1 cstate2 m). rewrite H7. simpl. reflexivity.
+Qed.
+
+Lemma chainstep_transform_next_block_valid
+    (cstate1 cstate2 : ChainState) 
+    (m : ChainStateMorphism cstate1 cstate2)
+    (header : BlockHeader) : 
+    IsValidNextBlock header cstate1 -> IsValidNextBlock header cstate2.
+Proof.
+    intro. destruct H7.
+    assert (env_chain cstate1 = env_chain cstate2); 
+    try exact (chain_eq' cstate1 cstate2 (env_morph cstate1 cstate2 m)).
+    rewrite H7 in valid_height.
+    rewrite H7 in valid_slot.
+    rewrite H7 in valid_finalized_height. 
+    exact (build_is_valid_next_block header cstate2 valid_height valid_slot valid_finalized_height valid_creator valid_reward).
+Qed.
+
+Lemma chainstep_transform_no_acts_from_accounts
+    (bstate1' : ChainState) : 
+    let bstate2' := bstate_transform_step bstate1' in  
+    Forall act_is_from_account (chain_state_queue bstate1') -> 
+    Forall act_is_from_account (chain_state_queue bstate2').
+Proof.
+    intros. 
+    unfold bstate2'.
+    simpl.
+    induction (chain_state_queue bstate1').
+    - auto.
+    - simpl. apply Forall_cons_iff in H7. destruct H7. apply IHl in H8.
+        apply Forall_cons.
+        + exact H7.
+        + exact H8.
+Qed.
+
+Lemma chainstep_transform_origin_eq_from
+    (bstate1' : ChainState) : 
+    let bstate2' := bstate_transform_step bstate1' in  
+    Forall act_origin_is_eq_from (chain_state_queue bstate1') -> 
+    Forall act_origin_is_eq_from (chain_state_queue bstate2').
+Proof.
+    intros. 
+    unfold bstate2'.
+    simpl.
+    induction (chain_state_queue bstate1').
+    - auto.
+    - simpl. apply Forall_cons_iff in H7. destruct H7. apply IHl in H8.
+        apply Forall_cons.
+        + exact H7.
+        + exact H8.
+Qed.
+
+Lemma chainstep_transform_step_env_chain_eq
+    (bstate1 bstate2 : ChainState)
+    (c_morph : ChainStateMorphism bstate1 bstate2) : 
+    env_chain bstate1 = env_chain bstate2.
+Proof.
+    exact (chain_eq' bstate1 bstate2 (env_morph bstate1 bstate2 c_morph)).
+Qed.
+
+Lemma env_equiv_carries_over_env_morphism 
+    (bstate1 bstate1' bstate2 bstate2' : Environment)
+    (e_morph  : EnvironmentMorphism bstate1  bstate2)
+    (e_morph' : EnvironmentMorphism bstate1' bstate2') :
+    EnvironmentEquiv bstate1 bstate1' -> 
+    EnvironmentEquiv bstate2 bstate2'.
+Proof.
+    intro EE1. destruct EE1. 
+    (* prove chain_eq *)
+    assert (env_chain bstate2 = env_chain bstate2').
+    rewrite (chain_eq' bstate1  bstate2  e_morph)  in chain_eq.
+    rewrite (chain_eq' bstate1' bstate2' e_morph') in chain_eq.
+    exact chain_eq.
+    (* prove account_balances_eq *)
+    assert (forall a, env_account_balances bstate2 a = env_account_balances bstate2' a).
+    intro.
+    rewrite <- (account_balances_eq' bstate1  bstate2  e_morph  a).
+    rewrite <- (account_balances_eq' bstate1' bstate2' e_morph' a).
+    exact (account_balances_eq a).
+    (* prove contracts_eq *)
+    assert (forall a, env_contracts bstate2 a = env_contracts bstate2' a).
+    intro.
+    rewrite (contracts_morph bstate1  bstate2  e_morph  a).
+    rewrite (contracts_morph bstate1' bstate2' e_morph' a).
+    rewrite <- (contracts_eq a). reflexivity.
+    (* prove contract_states_eq *)
+    assert (forall a, env_contract_states bstate2 a = env_contract_states bstate2' a).
+    intro.
+    rewrite (contract_states_morph bstate1  bstate2  e_morph  a).
+    rewrite (contract_states_morph bstate1' bstate2' e_morph' a).
+    rewrite <- (contracts_eq a).
+    rewrite <- (contract_states_eq a). reflexivity.
+    (* construct the result *)
+    exact {| chain_eq := H7 ; 
+             account_balances_eq := H8 ;
+             contracts_eq := H9 ;
+             contract_states_eq := H10 ; |}.
+Qed.
+
+(* then prove that adding a block preserves the cstate morphism *)
+Lemma env_morph_preserved_under_adding_block 
+    (bstate1 bstate2 : ChainState)
+    (e_morph : EnvironmentMorphism bstate1 bstate2)
+    (header : BlockHeader) : 
+    let bstate1' := (add_new_block_to_env header bstate1) in 
+    let bstate2' := (add_new_block_to_env header bstate2) in 
+    EnvironmentMorphism bstate1' bstate2'.
+Proof.
+    intros.
+    (* prove chain_eq' *)
+    assert (env_chain bstate1' = env_chain bstate2'). auto.
+    (* prove account_balances_eq' *)
+    assert (forall a, 
+        env_account_balances bstate1' a = env_account_balances bstate2' a).
+    unfold bstate1'. unfold bstate2'.
+    unfold add_new_block_to_env. 
+    intro. simpl.
+    rewrite <- (account_balances_eq' bstate1 bstate2 e_morph a). reflexivity.
+    (* prove contracts_morph *)
+    assert (forall a, 
+        env_contracts bstate2' a = 
+        match env_contracts bstate1' a with 
+        | Some wc => 
+            if (wc =? contract_to_weak_contract C1)%wc 
+            then Some (contract_to_weak_contract C2) 
+            else Some wc
+        | None => None 
+        end). 
+    unfold bstate1'. unfold bstate2'.
+    unfold add_new_block_to_env. 
+    intro. simpl. 
+    exact (contracts_morph bstate1 bstate2 e_morph a).
+    (* prove contract_states_morph *)
+    assert (forall a, 
+        env_contract_states bstate2' a = 
+        match env_contracts bstate1' a with 
+        | Some wc => 
+            if (wc =? contract_to_weak_contract C1)%wc 
+            then (option_fun (serialize_function state_morph)) (env_contract_states bstate1' a)
+            else env_contract_states bstate1' a
+        | None => env_contract_states bstate1' a
+        end).
+    unfold bstate1'. unfold bstate2'.
+    unfold add_new_block_to_env. 
+    intro. simpl. 
+    exact (contract_states_morph bstate1 bstate2 e_morph a).
+    (* construct the result *)
+    exact {| chain_eq' := H7 ; 
+             account_balances_eq' := H8 ;
+             contracts_morph := H9 ;
+             contract_states_morph := H10 ; |}.
+Qed.
+
+Lemma chainstep_transform_new_env_equiv_add_block
+    (bstate1 bstate2 bstate1' : ChainState)
+    (e_morph : EnvironmentMorphism bstate1 bstate2) 
+    (header : BlockHeader) : 
+    let bstate2' := bstate_transform_step bstate1' in  
+    EnvironmentEquiv bstate1' (add_new_block_to_env header bstate1) -> 
+    EnvironmentEquiv bstate2' (add_new_block_to_env header bstate2).
+Proof.
+    intros bstate2' EE1.
+    assert (EnvironmentMorphism (add_new_block_to_env header bstate1) (add_new_block_to_env header bstate2)); 
+    try exact (env_morph_preserved_under_adding_block bstate1 bstate2 e_morph header).
+    assert (EnvironmentMorphism bstate1' bstate2');
+    try exact (env_morph_step bstate1').
+    exact (symmetry (env_equiv_carries_over_env_morphism
+        (add_new_block_to_env header bstate1) bstate1'
+        (add_new_block_to_env header bstate2) bstate2'
+        H7 H8  (symmetry EE1))).
+Qed.
+
+Lemma permutation_preserved_over_map {A B : Type} : 
+    forall (g : A -> B) (l1 l2 : list A),
+    Permutation l1 l2 -> 
+    Permutation (List.map g l1) (List.map g l2).
+Proof.
+    intros.
+    induction H7.
+    - auto.
+    - simpl. exact (perm_skip (g x) IHPermutation).
+    - simpl. exact (perm_swap (g x) (g y) (map g l)).
+    - exact (perm_trans IHPermutation1 IHPermutation2).
+Qed.
+
+Lemma chainstep_transform_new_permuted 
+    (bstate1 bstate2 bstate1' : ChainState)
+    (env_equiv : EnvironmentEquiv bstate1 bstate1') 
+    (c_morph : ChainStateMorphism bstate1 bstate2) : 
+    let bstate2' := bstate_transform_step bstate1' in 
+    Permutation (chain_state_queue bstate1) (chain_state_queue bstate1') -> 
+    Permutation (chain_state_queue bstate2) (chain_state_queue bstate2').
+Proof.
+    intros.
+    simpl. rewrite (queue_morph bstate1 bstate2 c_morph).
+    assert (action_transform bstate1 = action_transform bstate1').
+    - apply functional_extensionality. intro a.
+        unfold action_transform. f_equal.
+        destruct (act_body a); auto.
+        rewrite (contracts_eq bstate1 bstate1' env_equiv to). auto.
+    - rewrite <- H8. 
+        exact (permutation_preserved_over_map (action_transform bstate1) (chain_state_queue bstate1) (chain_state_queue bstate1') H7).
+Qed.
+
+Lemma chainstep_transform_new_env_equiv_permute 
+    (bstate1 bstate2 bstate1' : ChainState)
+    (e_morph : EnvironmentMorphism bstate1 bstate2) : 
+    let bstate2' := bstate_transform_step bstate1' in 
+    EnvironmentEquiv bstate1' bstate1 -> 
+    EnvironmentEquiv bstate2' bstate2.
+Proof.
+    intros bstate2' EE1.
+    exact 
+    (symmetry
+    (env_equiv_carries_over_env_morphism 
+        bstate1 bstate1' bstate2 bstate2' 
+        e_morph
+        (env_morph_step bstate1')
+        (symmetry EE1))).
+Qed.
+
+Lemma chainstep_transform_new_queue_prev 
+    (bstate1 bstate2 : ChainState)
+    (c_morph : ChainStateMorphism bstate1 bstate2) : 
+    forall (act : Action) (acts : list Action),
+    chain_state_queue bstate1 = act :: acts -> 
+    let new_act := action_transform bstate1 act in 
+    let new_acts := List.map (action_transform bstate1) acts in
+    chain_state_queue bstate2 = new_act :: new_acts.
+Proof.
+    intros.
+    unfold new_act. unfold new_acts.
+    rewrite (queue_morph bstate1 bstate2 c_morph). 
+    rewrite H7.
+    auto.
+Qed.
+
+Lemma chainstep_transform_new_act_eval_true 
+    (bstate1 bstate2 bstate1' : ChainState)
+    (c_morph : ChainStateMorphism bstate1 bstate2) : 
+    forall (act : Action) (new_acts : list Action),
+    let act' := action_transform bstate1 act in
+    let new_acts' := List.map (action_transform bstate1') new_acts in
+    let bstate2' := bstate_transform_step bstate1' in
+    ActionEvaluation bstate1 act  bstate1' new_acts ->
+    ActionEvaluation bstate2 act' bstate2' new_acts'.
+Proof. Admitted.
+
+(* TODO transform bstate back *)
+Lemma act_eval_pullback 
+    (bstate1 bstate2 : ChainState) 
+    (c_morph : ChainStateMorphism bstate1 bstate2)
+    (bstate : Environment) (act : Action) (new_acts : list Action) : 
+    let act' := action_transform bstate1 act in 
+    ActionEvaluation bstate2 act' bstate new_acts ->
+    ActionEvaluation bstate1 act  bstate new_acts.
+Proof. Admitted.
+
+Lemma chainstep_transform_new_act_eval_false
+    (bstate1 bstate2 : ChainState) 
+    (c_morph : ChainStateMorphism bstate1 bstate2)
+    (act : Action) : 
+    let act' := action_transform bstate1 act in 
+    (forall bstate new_acts, ActionEvaluation bstate1 act  bstate new_acts -> False) ->
+    (forall bstate new_acts, ActionEvaluation bstate2 act' bstate new_acts -> False).
+Proof.
+    intros.
+    apply (H7 bstate new_acts).
+    apply (act_eval_pullback bstate1 bstate2 c_morph bstate act new_acts).
+    exact X.
+Qed.
+
+Lemma list_map_concat {A B : Type} {g : A -> B} : 
+    forall (l1 l2 : list A), 
+    List.map g (l1 ++ l2) = (List.map g l1) ++ (List.map g l2).
+Proof.
+    intros. 
+    induction l1.
+    - auto.
+    - assert (((a :: l1) ++ l2) = a :: (l1 ++ l2)); auto. rewrite H7.
+        assert (forall a' k, map g (a' :: k) = (g a') :: map g k); auto. 
+        rewrite (H8 a (l1 ++ l2)).
+        rewrite (H8 a l1).
+        assert (forall (a':B) k1 k2, (a' :: k1) ++ k2 = a' :: (k1 ++ k2)); auto.
+        rewrite (H9 (g a) (map g l1) (map g l2)).
+        rewrite IHl1. reflexivity.
+Qed.
+
+Lemma chainstep_transform_new_queue_next
+    (bstate1 bstate2 bstate1' : ChainState)
+    (c_morph : ChainStateMorphism bstate1 bstate2) : 
+    forall (new_acts : list Action) (acts : list Action),
+    chain_state_queue bstate1' = new_acts ++ acts -> 
+    let bstate2'  := bstate_transform_step bstate1' in  
+    let new_acts' := List.map (action_transform bstate1') new_acts in 
+    let acts'     := List.map (action_transform bstate1) acts in
+    chain_state_queue bstate2' = new_acts' ++ acts'.
+Proof.
+    intros.
+    unfold bstate2'.
+    unfold bstate_transform_step. simpl.
+    unfold new_acts'. unfold acts'. rewrite H7.
+    rewrite (list_map_concat new_acts acts). 
+    f_equal.
+    admit.
+Admitted.
+
+Lemma chainstep_transform_queue_next_action_invalid
+    (bstate1 bstate2 bstate1' : ChainState) 
+    (acts : list Action): 
+    let bstate2' := bstate_transform_step bstate1' in  
+    let acts' := List.map (action_transform bstate1) acts in 
+    chain_state_queue bstate1' = acts ->
+    chain_state_queue bstate2' = acts'.
+Proof.
+    intros.
+    unfold bstate2'. 
+    unfold bstate_transform_step. simpl.
+    unfold acts'. rewrite H7.
+    admit.
+Admitted.
+
+Lemma chainstep_transform_from_acct
+    (bstate : ChainState) (act : Action) : 
+    act_is_from_account act -> 
+    act_is_from_account (action_transform bstate act).
+Proof.
+    unfold act_is_from_account.
+    intros.
+    assert (act_from (action_transform bstate act) = act_from act).
+    - unfold action_transform. auto.
+    - rewrite H8. exact H7.
+Qed.
+
+Definition chainstep_transform_step 
+    (bstate1 bstate2 bstate1' : ChainState)
+    (c_morph : ChainStateMorphism bstate1 bstate2) 
+    (step : ChainStep bstate1 bstate1') : 
+    let bstate2' := bstate_transform_step bstate1' in  
+    (ChainStep bstate2 bstate2') :=
+    let bstate2' := bstate_transform_step bstate1' in  
+    let c_morph' := chainstate_morphism_step bstate1' in 
+    match step with 
+    | step_block _ _ header prev_queue_empty next_block_valid no_acts_from_accounts origin_eq_from 
+        env_equiv  => 
+        (* modified header *)
+        let header' := header in 
+        (* modified prev_queue_empty *)
+        let prev_queue_empty' := 
+            chainstep_transform_empty_queue bstate1 bstate2 c_morph prev_queue_empty in 
+        (* modified next_block_valid *)
+        let next_block_valid' := 
+            chainstep_transform_next_block_valid bstate1 bstate2 c_morph header next_block_valid in 
+        (* modified no_acts_from_accounts *)
+        let no_acts_from_accounts' := 
+            chainstep_transform_no_acts_from_accounts bstate1' no_acts_from_accounts in
+        (* modified origin_eq_from *)
+        let origin_eq_from' :=
+            chainstep_transform_origin_eq_from bstate1' origin_eq_from in 
+        (* modified env_equiv *)
+        let env_equiv' :=
+            chainstep_transform_new_env_equiv_add_block bstate1 bstate2 bstate1' 
+            (env_morph bstate1 bstate2 c_morph) header env_equiv in
+        (* the new step_block *)
+        step_block bstate2 bstate2'
+            header' prev_queue_empty' next_block_valid' no_acts_from_accounts' 
+            origin_eq_from' env_equiv'
+    | step_action _ _ act acts new_acts queue_prev act_eval_true queue_next => 
+        (* modified act *)
+        let act' := action_transform bstate1 act in 
+        (* modified acts *)
+        let acts' := 
+            List.map (action_transform bstate1) acts in 
+        (* modified new_acts *)
+        let new_acts' := 
+            List.map (action_transform bstate1') new_acts in 
+        (* modified queue_prev *)
+        let queue_prev' := 
+            chainstep_transform_new_queue_prev bstate1 bstate2 c_morph act acts queue_prev in 
+        (* modified act_eval_true *)
+        let act_eval_true' := 
+            chainstep_transform_new_act_eval_true bstate1 bstate2 bstate1' c_morph act new_acts act_eval_true in 
+        (* modified queue_next *)
+        let queue_next' := 
+            chainstep_transform_new_queue_next bstate1 bstate2 bstate1' c_morph new_acts acts queue_next in
+        (* the new step_block *)
+        step_action bstate2 bstate2' act' acts' new_acts' queue_prev' act_eval_true' queue_next'
+    | step_action_invalid _ _ act acts env_equiv queue_prev queue_next from_acct actn_eval_false => 
+        (* modified act *)
+        let act' := action_transform bstate1 act in 
+        (* modified acts *)
+        let acts' := 
+            List.map (action_transform bstate1) acts in 
+        (* modified env_equiv *)
+        let env_equiv' := 
+            chainstep_transform_new_env_equiv_permute bstate1 bstate2 bstate1' 
+            (env_morph bstate1 bstate2 c_morph) env_equiv in 
+        (* modified queue_prev *)
+        let queue_prev' := 
+            chainstep_transform_new_queue_prev bstate1 bstate2 c_morph act acts queue_prev in 
+        (* modified queue_next *)
+        let queue_next' := 
+            chainstep_transform_queue_next_action_invalid bstate1 bstate2 bstate1' acts queue_next in 
+        (* modified from_acct *)
+        let from_acct' := 
+            chainstep_transform_from_acct bstate1 act from_acct in 
+        (* modified actn_eval_false *)
+        let actn_eval_false' := 
+            chainstep_transform_new_act_eval_false bstate1 bstate2 c_morph act actn_eval_false in 
+        (* the new step_block *)
+        step_action_invalid bstate2 bstate2' act' acts' env_equiv' queue_prev' queue_next' from_acct' actn_eval_false'
+    | step_permute _ _ env_equiv permuted => 
+        (* modified env_equiv *)
+        let env_equiv' := 
+            chainstep_transform_new_env_equiv_permute bstate1 bstate2 bstate1' 
+            (env_morph bstate1 bstate2 c_morph) env_equiv in 
+        (* modified permutation *)
+        let permuted' := 
+            chainstep_transform_new_permuted bstate1 bstate2 bstate1' (symmetry env_equiv) c_morph permuted in 
+        (* the new step_block *)
+        step_permute bstate2 bstate2' env_equiv' permuted' 
+    end.
+
+Definition caddr_implication_step (bstate1' : ChainState) (caddr : Address) :
+    let bstate2' := bstate_transform_step bstate1' in  
+    env_contracts bstate1' caddr = Some (C1 : WeakContract) -> 
+    env_contracts bstate2' caddr = Some (C2 : WeakContract).
+Proof.
+    intros. unfold bstate2'.
+    unfold bstate_transform_step. simpl.
+    rewrite H7. 
+    destruct (C1 =? C1)%wc; auto.
+    contradiction.
+Qed.
+
+End CMLiftInductiveStep.
+
+(* Theorem: A contract morphism can be lifted into a morphism of ChainStates *)
+Theorem cm_lift :
+    forall  bstate1 caddr (trace : ChainTrace empty_state bstate1),
+    exists  (* a new bstate related to the old *)
+            (bstate2 : ChainState) 
+            (bstate_morph : ChainStateMorphism bstate1 bstate2)
+            (* a new trace constructed from the old *)
+            (trace2 : ChainTrace empty_state bstate2),
+            (* with C2 swapped out for C1 *)
+            env_contracts bstate1 caddr = Some (C1 : WeakContract) -> 
+            env_contracts bstate2 caddr = Some (C2 : WeakContract).
+Proof.
+    (* we induct over the trace *)
+    intros.
+    remember empty_state eqn:genesis_empty. 
+    induction trace.
+    - rewrite genesis_empty. 
+        exists empty_state. 
+        exists empty_chainstate_morphism. 
+        exists ChainedList.clnil.
+        intro. assert (env_contracts empty_state caddr = None); auto. 
+        rewrite H8 in H7. congruence.
+    - apply IHtrace in genesis_empty. clear IHtrace.
+        destruct genesis_empty as [bstate2 genesis_empty]. 
+        destruct genesis_empty as [bstate_morph genesis_empty]. 
+        destruct genesis_empty as [trace2 addr_implication].
+        (* construct the new bstate and trace *)
+        set (bstate2' := bstate_transform_step to).
+        set (l' := chainstep_transform_step mid bstate2 to bstate_morph l).
+        set (trace2' := ChainedList.snoc trace2 l').
+        (* construct the relationships *)
+        set (bstate_morph' := chainstate_morphism_step to).
+        set (caddr_impl := caddr_implication_step to caddr).
+        exists bstate2'. 
+        exists bstate_morph'. 
+        exists trace2'.
+        exact caddr_impl.
+Qed.
+
+(* TODO a non-opaque construction? *)
+
+End ContractMorphismLift.
+
+
+(** We now examin how lifted morphisms behave with regard to morphism composition *)
+Section ContractMorphismLiftCompose.
+
+(*
+Lemma id_lifts_to_id 
+
+Lemma morphisms_lift_compose
+
+Lemma iso_lifts_to_iso
+
+Lemma inj_lifts_to_inj
+
+Lemma surj_lifts_to_surj
+*)
+
+End ContractMorphismLiftCompose.
 
 End ContractMorphisms.
